@prefix :      <http://www.w3.org/2002/07/owl#> .
@prefix home:  <http://sensormeasurement.appspot.com/home#> .
@prefix ucum:  <http://idi.fundacionctic.org/muo/ucum-instances.owl> .
@prefix ssn:   <http://purl.oclc.org/NET/ssnx/ssn#> .
@prefix vann:  <http://purl.org/vocab/vann/> .
@prefix vs:    <http://www.w3.org/2003/06/sw-vocab-status/ns#> .
@prefix qudt_unit: <http://data.qudt.org/qudt/owl/1.0.0/unit.owl#> .
@prefix qudt:  <http://qudt.org/schema/qudt#> .
@prefix dogont: <http://elite.polito.it/ontologies/dogont.owl#> .
@prefix dcterms: <http://purl.org/dc/terms/> .
@prefix rdfs:  <http://www.w3.org/2000/01/rdf-schema#> .
@prefix txn:   <http://lod.taxonconcept.org/ontology/txn.owl#> .
@prefix m3-lite: <http://purl.org/iot/vocab/m3-lite#> .
@prefix dbpedia: <http://dbpedia.org/ontology/> .
@prefix weather: <http://archive.knoesis.org/research/semsci/application_domain/sem_sensor/ont/weather.owl> .
@prefix rdf:   <http://www.w3.org/1999/02/22-rdf-syntax-ns#> .
@prefix cose:  <http://casas.wsu.edu/owl/cose.owl#> .
@prefix qu:    <http://purl.org/NET/ssnx/qu/qu#> .
@prefix dc:    <http://purl.org/dc/elements/1.1/> .
@prefix spitfire: <http://spitfire-project.eu/ontology/ns/> .
@prefix mo:    <http://purl.org/ontology/mo/> .
@prefix wgs84_pos: <http://www.w3.org/2003/01/geo/wgs84_pos#> .
@prefix foaf:  <http://xmlns.com/foaf/0.1/> .
@prefix iot-lite: <http://purl.oclc.org/NET/UNIS/fiware/iot-lite#> .
@prefix sweet_unit: <http://sweet.jpl.nasa.gov/ontology/units.owl#> .
@prefix emoca: <http://ns.inria.fr/emoca#> .
@prefix movie: <http://www.movieontology.org/2010/01/movieontology.owl> .
@prefix ontoSensor: <http://mmisw.org/ont/univmemphis/sensor> .
@prefix openIoT: <http://openiot.eu/ontology/ns/> .
@prefix qu_rec20: <http://purl.org/NET/ssnx/qu/qu-rec20#> .
@prefix shw:   <http://paul.staroch.name/thesis/SmartHomeWeather.owl#> .
@prefix muo:   <http://purl.oclc.org/NET/muo/muo#> .
@prefix voaf:  <http://purl.org/vocommons/voaf#> .
@prefix aws:   <http://purl.oclc.org/NET/ssnx/meteo/aws#> .
@prefix naturopathy: <http://sensormeasurement.appspot.com/naturopathy#> .
@prefix dul:   <http://www.loa-cnr.it/ontologies/DUL.owl#> .
@prefix xsd:   <http://www.w3.org/2001/XMLSchema#> .
@prefix owl:   <http://www.w3.org/2002/07/owl#> .
@prefix food_smart_product: <http://kmi.open.ac.uk/projects/smartproducts/ontologies/food.owl#> .
@prefix cc:    <http://creativecommons.org/ns#> .

m3-lite:Air  a           owl:Class ;
        rdfs:comment     "Air as an IoT applicative domain"@en ;
        rdfs:label       "Air"@en ;
        rdfs:subClassOf  m3-lite:Environment .

m3-lite:Microgram  a     owl:Class ;
        rdfs:label       "Microgram (ug)" ;
        rdfs:subClassOf  m3-lite:Gram .

m3-lite:Index  a         owl:Class ;
        rdfs:comment     "Arbitrary indirect reference which should be translated into meaningful measurements by using the corresponding decoding algorithm detailed in the resource description. In this case the returned values can only take certain values from a finite set." ;
        rdfs:label       "Index"@en ;
        rdfs:subClassOf  qu:Unit .

m3-lite:OccupancyDetector
        a                owl:Class ;
        rdfs:comment     "Presence detector, motion sensor, Pyroelectric IR Occupancy Detector, Intrusion Detector/ Trespassing, Infrared Sensor, Proximity sensor are used to detect human location. Used in iPhone4 to detect whtn the user holds the phone to her face to speak to diable touchscreen."@en ;
        rdfs:label       "Presence Detector"@en ;
        rdfs:seeAlso     cose:PassiveInfraredSensor ;
        rdfs:subClassOf  ssn:SensingDevice ;
        rdfs:subClassOf  [ a                   owl:Restriction ;
                           owl:onProperty      m3-lite:domainOfInterest ;
                           owl:someValuesFrom  m3-lite:BuildingAutomation
                         ] .

m3-lite:PaymentCard  a   owl:Class ;
        rdfs:comment     "An RFID tag is embedded on payment card."@en ;
        rdfs:label       "Payment Card"@en ;
        rdfs:subClassOf  m3-lite:RFIDQuantityKind .

m3-lite:Minute_time  a   owl:Class ;
        rdfs:comment     ""@en ;
        rdfs:label       "Minute_time"@en ;
        rdfs:subClassOf  qu:Unit .

m3-lite:RoadOccupancy
        a                owl:Class ;
        rdfs:comment     "Ratio of time on which a road lane section is occupied by vehicles within a given period of time." ;
        rdfs:label       "Road Occupancy"@en ;
        rdfs:subClassOf  qu:QuantityKind .

m3-lite:PresenceStateParking
        a                owl:Class ;
        rdfs:comment     "The presence or absence of a vehicle parked." ;
        rdfs:label       "Presence State Parking"@en ;
        rdfs:subClassOf  m3-lite:PresenceState .

m3-lite:TrackingPaymentCard
        a                owl:Class ;
        rdfs:comment     ""@en ;
        rdfs:label       "Tracking Payment Card"@en ;
        rdfs:subClassOf  m3-lite:TrackingGood .

m3-lite:FillLevel  a     owl:Class ;
        rdfs:label       "Fill Level"@en ;
        rdfs:subClassOf  qu:QuantityKind .

m3-lite:TimeRelatedStateDriver1
        a                owl:Class ;
        rdfs:comment     "Indicates if the first driver approaches or exceeds working time limits (or other limits)." ;
        rdfs:label       "Time Related State Driver 1"@en ;
        rdfs:subClassOf  m3-lite:TimeRelatedStateDriver .

m3-lite:SunPositionDirectionSensor
        a                owl:Class ;
        rdfs:comment     "To detect sun from north eastm, south or west. Unit Degree"@en ;
        rdfs:label       "Sun Position Direction Sensor"@en ;
        rdfs:subClassOf  ssn:SensingDevice ;
        rdfs:subClassOf  [ a                   owl:Restriction ;
                           owl:onProperty      m3-lite:domainOfInterest ;
                           owl:someValuesFrom  m3-lite:Weather
                         ] .

m3-lite:Scale  a         owl:Class ;
        rdfs:comment     "Arbitrary indirect reference which should be translated into meaningful measurements by using the corresponding decoding algorithm detailed in the resource description. In this case the returned values are part of a continuous variable which can take any numeric value." ;
        rdfs:label       "Scale"@en ;
        rdfs:subClassOf  qu:Unit .

m3-lite:MillimeterPerHour
        a                owl:Class ;
        rdfs:comment     "One millimetre of rainfall is the equivalent of one litre of water per square metre in one hour." ;
        rdfs:label       "MillimeterPerHour, MillimetrePerHour" ;
        rdfs:seeAlso     "http://purl.oclc.org/NET/ssnx/qu/unit#millimetrePerHour" ;
        rdfs:subClassOf  qu:Unit .

m3-lite:FoodTemperature
        a                owl:Class ;
        rdfs:comment     ""@en ;
        rdfs:label       "Food Temperature"@en ;
        rdfs:subClassOf  m3-lite:Temperature .

m3-lite:KilogramPerCubicMetre
        a                owl:Class ;
        rdfs:label       "KilogramPerCubicMetre, KilogramPerCubicMeter" ;
        rdfs:subClassOf  m3-lite:GramPerCubicMetre .

owl:equivalentClass  a  owl:AnnotationProperty .

m3-lite:GyroscopeSensor
        a                owl:Class ;
        rdfs:comment     "A gyroscope is a device for measuring or maintening orientation. In a home it can be attached to a broom, mop, etc. Used in iPhone 4."@en ;
        rdfs:label       "Gyroscope Sensor"@en ;
        rdfs:seeAlso     cose:Gyroscope ;
        rdfs:subClassOf  ssn:SensingDevice ;
        rdfs:subClassOf  [ a                   owl:Restriction ;
                           owl:onProperty      m3-lite:domainOfInterest ;
                           owl:someValuesFrom  m3-lite:Transportation
                         ] ;
        rdfs:subClassOf  [ a                   owl:Restriction ;
                           owl:onProperty      m3-lite:domainOfInterest ;
                           owl:someValuesFrom  m3-lite:BuildingAutomation
                         ] .

m3-lite:PresenceStateEmergencyVehicle
        a                owl:Class ;
        rdfs:comment     "The presence or absence of an emergency vehicle (ambulance, fire fighters, etc.)." ;
        rdfs:label       "Presence State Emergency Vehicle"@en ;
        rdfs:subClassOf  m3-lite:PresenceState .

m3-lite:MmHg  a          owl:Class ;
        rdfs:comment     "mmHg unit is used to measure blood pressure measurements (systolic and diastolic)."@en ;
        rdfs:label       "mmHg"@en ;
        rdfs:subClassOf  qu:Unit .

m3-lite:Microwave  a     owl:Class ;
        rdfs:comment     "An actuator to automatically switch on/off the Microwave."@en ;
        rdfs:label       "Microwave"@en ;
        rdfs:subClassOf  iot-lite:ActuatingDevice ;
        rdfs:subClassOf  [ a                   owl:Restriction ;
                           owl:onProperty      m3-lite:domainOfInterest ;
                           owl:someValuesFrom  m3-lite:BuildingAutomation
                         ] .

m3-lite:Telephone  a     owl:Class ;
        rdfs:comment     "An actuator to automatically switch on/off the Telephone."@en ;
        rdfs:label       "Telephone"@en ;
        rdfs:subClassOf  iot-lite:ActuatingDevice ;
        rdfs:subClassOf  [ a                   owl:Restriction ;
                           owl:onProperty      m3-lite:domainOfInterest ;
                           owl:someValuesFrom  m3-lite:BuildingAutomation
                         ] .

m3-lite:Environment  a   owl:Class ;
        rdfs:comment     "Environment (earthquake, flooding, fire, pollution) as an Internet of Things (IoT) applicative domain."@en ;
        rdfs:label       "Environment"@en ;
        rdfs:subClassOf  m3-lite:DomainOfInterest .

m3-lite:WindChill  a     owl:Class ;
        rdfs:comment     "Wind chill"@en ;
        rdfs:label       "Wind chill"@en ;
        rdfs:seeAlso     openIoT:WindChill ;
        rdfs:subClassOf  qu:QuantityKind .

m3-lite:TimeRelatedStateDriver
        a                owl:Class ;
        rdfs:label       "Time Related State Driver"@en ;
        rdfs:subClassOf  m3-lite:TimeRelatedState .

m3-lite:Cupboard  a      owl:Class ;
        rdfs:comment     "An actuator to automatically open/close the cupboard."@en ;
        rdfs:label       "Cupboard"@en ;
        rdfs:subClassOf  iot-lite:ActuatingDevice ;
        rdfs:subClassOf  [ a                   owl:Restriction ;
                           owl:onProperty      m3-lite:domainOfInterest ;
                           owl:someValuesFrom  m3-lite:BuildingAutomation
                         ] .

m3-lite:Luggage  a       owl:Class ;
        rdfs:comment     "An RFID tag is embedded on luggage."@en ;
        rdfs:label       "Luggage"@en ;
        rdfs:subClassOf  m3-lite:RFIDQuantityKind .

m3-lite:MilligramPerSquareMetre
        a                owl:Class ;
        rdfs:comment     "A dose unit which is equal to 1 milligram of a toxic or pharmaceutical substance per square meter of surface area of the recipient subject." ;
        rdfs:label       "Milligram Per Square Metre" ;
        rdfs:seeAlso     "http://purl.oclc.org/NET/ssnx/qu/unit#milligramPerSquareMetre" ;
        rdfs:subClassOf  qu:Unit .

m3-lite:TemperatureWasteContainer
        a                owl:Class ;
        rdfs:comment     "The temperature of the air that would be indicated by a thermometer exposed to the air inside a waste container." ;
        rdfs:label       "Waste Container" ;
        rdfs:subClassOf  m3-lite:Temperature .

m3-lite:Blind  a         owl:Class ;
        rdfs:comment     "An actuator to automatically switch on/off the blind."@en ;
        rdfs:label       "Blind"@en ;
        rdfs:subClassOf  iot-lite:ActuatingDevice ;
        rdfs:subClassOf  [ a                   owl:Restriction ;
                           owl:onProperty      m3-lite:domainOfInterest ;
                           owl:someValuesFrom  m3-lite:BuildingAutomation
                         ] .

m3-lite:Sodium  a        owl:Class ;
        rdfs:comment     "Blood Sodium level"@en ;
        rdfs:label       "Sodium"@en ;
        rdfs:subClassOf  qu:QuantityKind .

txn:hasImage  a  owl:AnnotationProperty .

m3-lite:Activity  a      owl:Class ;
        rdfs:comment     "Activity recognition as an IoT applicative domain"@en ;
        rdfs:label       "Activity recognition"@en ;
        rdfs:subClassOf  m3-lite:BuildingAutomation .

m3-lite:Percent  a       owl:Class ;
        rdfs:comment     ""@en ;
        rdfs:label       "Percent"@en ;
        rdfs:seeAlso     sweet_unit:percent , qudt_unit:Percent ;
        rdfs:subClassOf  qu:Unit .

m3-lite:Barcode  a       owl:Class ;
        rdfs:comment     "A tagging device can be Barcode"@en ;
        rdfs:label       "Barcode"@en ;
        rdfs:subClassOf  iot-lite:TagDevice .

m3-lite:Degree  a        owl:Class ;
        rdfs:subClassOf  qu:Unit .

m3-lite:Boiler  a        owl:Class ;
        rdfs:comment     "An actuator to automatically switch on/off the boiler."@en ;
        rdfs:label       "Boiler"@en ;
        rdfs:subClassOf  iot-lite:ActuatingDevice ;
        rdfs:subClassOf  [ a                   owl:Restriction ;
                           owl:onProperty      m3-lite:domainOfInterest ;
                           owl:someValuesFrom  m3-lite:BuildingAutomation
                         ] .

m3-lite:DomainOfInterest
        a       owl:Class .

m3-lite:SpeedMedian  a   owl:Class ;
        rdfs:comment     "A measure of the median rate of motion of an object." ;
        rdfs:label       "Speed Median"@en ;
        rdfs:subClassOf  m3-lite:Speed .

m3-lite:TrackingLuggage
        a                owl:Class ;
        rdfs:comment     ""@en ;
        rdfs:label       "Tracking Luggage"@en ;
        rdfs:subClassOf  m3-lite:TrackingGood .

m3-lite:Decibel  a       owl:Class ;
        rdfs:comment     "A ratio unit which is an indicator of sound power per unit area."@en ;
        rdfs:label       "Decibel (db)"@en ;
        rdfs:seeAlso     "http://purl.oclc.org/NET/ssnx/qu/unit#decibel" ;
        rdfs:subClassOf  qu:Unit .

m3-lite:ActivePower  a   owl:Class ;
        rdfs:comment     "The product of the voltage across a branch of an alternating-current circuit and the component of the electric current that is in phase with the voltage." ;
        rdfs:seeAlso     "http://purl.oclc.org/NET/ssnx/qu/quantity#activePower" ;
        rdfs:subClassOf  m3-lite:Power .

m3-lite:Hydrophone  a    owl:Class ;
        rdfs:comment     "A hydrophone is a microphone designed to be used underwater for recording or listening to underwater sound."@en ;
        rdfs:label       "Hydrophone"@en ;
        rdfs:subClassOf  ssn:SensingDevice .

m3-lite:TrackingGood  a  owl:Class ;
        rdfs:comment     "Tracking RFID Goods as an Internet of Things (IoT) applicative domain."@en ;
        rdfs:label       "Tracking RFID Goods"@en ;
        rdfs:subClassOf  m3-lite:DomainOfInterest .

m3-lite:RadianPerSecond
        a                owl:Class ;
        rdfs:comment     "The radian per second is defined as the change in the orientation of an object, in radians, every second. The radian per second is the SI unit of angular (rotational) speed." ;
        rdfs:label       "Radian Per Second"@en ;
        rdfs:seeAlso     "http://purl.oclc.org/NET/ssnx/qu/unit#radianPerSecond" ;
        rdfs:subClassOf  qu:Unit .

m3-lite:AlcoholLevelSensor
        a                owl:Class ;
        rdfs:comment     "Alcohol Level Sensor"@en ;
        rdfs:label       "Alcohol Level Sensor"@en ;
        rdfs:subClassOf  ssn:SensingDevice ;
        rdfs:subClassOf  [ a                   owl:Restriction ;
                           owl:onProperty      m3-lite:domainOfInterest ;
                           owl:someValuesFrom  m3-lite:Transportation
                         ] ;
        txn:hasImage     <http://sensormeasurement.appspot.com/images/sensor/noise.png> .

m3-lite:CloudCoverSensor
        a                owl:Class ;
        rdfs:comment     "Cloud Cover Sensor is used to detect whater is is sunny, cloudy, etc. It is measured in okta."@en ;
        rdfs:label       "Cloud Cover Sensor"@en ;
        rdfs:subClassOf  ssn:SensingDevice ;
        rdfs:subClassOf  [ a                   owl:Restriction ;
                           owl:onProperty      m3-lite:domainOfInterest ;
                           owl:someValuesFrom  m3-lite:Weather
                         ] ;
        txn:hasImage     <http://sensormeasurement.appspot.com/images/sensor/cloud.png> .

iot-lite:TagDevice  a    owl:Class ;
        rdfs:comment     "A tagging device can be RFID, QRCode, NFC, Barcode, etc."@en ;
        rdfs:label       "Tagging Device"@en ;
        rdfs:subClassOf  ssn:Device .

m3-lite:Tourism  a       owl:Class ;
        rdfs:comment     "Tourism as an Internet of Things (IoT) applicative domain."@en ;
        rdfs:label       "Tourism"@en ;
        rdfs:subClassOf  m3-lite:DomainOfInterest .

m3-lite:Visibility  a    owl:Class ;
        rdfs:comment     ""@en ;
        rdfs:label       "Visibility"@en ;
        rdfs:seeAlso     openIoT:AtmosphereVisibility ;
        rdfs:subClassOf  qu:QuantityKind .

m3-lite:CholesterolSensor
        a                owl:Class ;
        rdfs:comment     "Cholesterol Sensor"@en ;
        rdfs:label       "Cholesterol Sensor"@en ;
        rdfs:subClassOf  ssn:SensingDevice ;
        rdfs:subClassOf  [ a                   owl:Restriction ;
                           owl:onProperty      m3-lite:domainOfInterest ;
                           owl:someValuesFrom  m3-lite:Health
                         ] ;
        txn:hasImage     <http://sensormeasurement.appspot.com/images/sensor/cholesterol.png> .

m3-lite:ElectricField2100MHz
        a                owl:Class ;
        rdfs:comment     "A field of force associated with a moving electric charge equivalent to an electric field and a magnetic field at right angles to each other and to the direction of propagation. Applied to the 2100 MHz UHF band." ;
        rdfs:label       "Electric Field 2100 MHz"@en ;
        rdfs:subClassOf  m3-lite:ElectricField .

m3-lite:LeafWetnessSensor
        a                owl:Class ;
        rdfs:comment     "Leaf Wetness Sensor is used in agriculture to check whether the plants need to be watered."@en ;
        rdfs:label       "Leaf Wetness Sensor"@en ;
        rdfs:subClassOf  ssn:SensingDevice ;
        rdfs:subClassOf  [ a                   owl:Restriction ;
                           owl:onProperty      m3-lite:domainOfInterest ;
                           owl:someValuesFrom  m3-lite:Agriculture
                         ] .

m3-lite:  a                            owl:Ontology ;
        rdfs:comment                   "M3 lite taxonomy is designed for the FIESTA-IOT H2020 EU project. We refactor, clean and simplify the M3 ontology designed by Eurecom (Amelie Gyrard). M3 ontology lite is currently aligned with the quantity taxonomy used by several testbeds: SmartSantander (Spain), University of Surrey (United Kingdom), KETI (Korea) and Com4Innov (France)."@en ;
        dc:creator                     "Luis Sanchez, UC, Santander"@en , "David Gomez, UC, Santander"@en , "Tarek Elsaleh, UNIS, Surrey"@en , "Rachit Agarwal, Inria, Paris"@en , "Amelie Gyrard, NUIG, Galway"@en ;
        dc:description                 "The Machine-to-Machine Measurement (M3) Ontology is an unified language, nomenclature, dictionary which enables semantically annotating heterogeneous IoT data produced by heterogeneous devices measurements (sensors, RFID tags, etc.). We classify all devices, their measurements and the feature of interests (health, smart home, smart kitchen, environmental monitoring, etc.). By combining data from heterogeneous areas, we could propose new kinds of applications."@en ;
        dc:title                       "The Machine-to-Machine Measurement (M3) Lite Ontology"@en ;
        dcterms:issued                 "2015-07-02"^^xsd:date ;
        dcterms:modified               "2016-04-25" ;
        vann:preferredNamespacePrefix  "m3-lite" ;
        vann:preferredNamespaceUri     "http://purl.org/iot/vocab/m3-lite#" ;
        owl:versionInfo                0.6 ;
        vs:term_status                 "Work in progress" .

m3-lite:Dimensionless
        a                owl:Class ;
        rdfs:comment     "Without dimensions; having no appreciable or noteworthy extent. Without physical meaning." ;
        rdfs:label       "Dimension less"@en ;
        rdfs:seeAlso     "http://purl.oclc.org/NET/ssnx/qu/dim#Dimensionless" ;
        rdfs:subClassOf  qu:Unit .

m3-lite:Tesla  a         owl:Class ;
        rdfs:comment     ""@en ;
        rdfs:label       "Tesla"@en ;
        rdfs:subClassOf  qu:Unit .

m3-lite:Salinity  a      owl:Class ;
        rdfs:comment     "Salinity"@en ;
        rdfs:label       "Salinity"@en ;
        rdfs:subClassOf  qu:QuantityKind .

m3-lite:Milligram  a     owl:Class ;
        rdfs:label       "Milligram (mg)" ;
        rdfs:subClassOf  m3-lite:Gram .

m3-lite:LeafWetness  a   owl:Class ;
        rdfs:comment     "Leaf Wetness"@en ;
        rdfs:label       "Leaf Wetness"@en ;
        rdfs:subClassOf  qu:QuantityKind .

m3-lite:Potassium  a     owl:Class ;
        rdfs:comment     "Blood Potassium level"@en ;
        rdfs:label       "Potassium"@en ;
        rdfs:subClassOf  qu:QuantityKind .

m3-lite:VisibilitySensor
        a                owl:Class ;
        rdfs:comment     "Visibility sensor to detect fog"@en ;
        rdfs:label       "Visibility Sensor"@en ;
        rdfs:subClassOf  ssn:SensingDevice ;
        rdfs:subClassOf  [ a                   owl:Restriction ;
                           owl:onProperty      m3-lite:domainOfInterest ;
                           owl:someValuesFrom  m3-lite:Transportation
                         ] .

m3-lite:PHSensor  a      owl:Class ;
        rdfs:comment     "PH Sensor"@en ;
        rdfs:label       "PH Sensor"@en ;
        rdfs:subClassOf  ssn:SensingDevice ;
        rdfs:subClassOf  [ a                   owl:Restriction ;
                           owl:onProperty      m3-lite:domainOfInterest ;
                           owl:someValuesFrom  m3-lite:Agriculture
                         ] .

m3-lite:Power  a         owl:Class ;
        rdfs:comment     ""@en ;
        rdfs:label       "Power"@en ;
        rdfs:subClassOf  qu:QuantityKind .

m3-lite:WaterFlow  a     owl:Class ;
        rdfs:comment     "Water flow to detect if sinks, showers, baths or flushing are used."@en ;
        rdfs:label       "Water Flow "@en ;
        rdfs:subClassOf  iot-lite:ActuatingDevice ;
        rdfs:subClassOf  [ a                   owl:Restriction ;
                           owl:onProperty      m3-lite:domainOfInterest ;
                           owl:someValuesFrom  m3-lite:BuildingAutomation
                         ] .

m3-lite:ElectricalResistance
        a                owl:Class ;
        rdfs:comment     "The electrical resitance of an electrical conductor is the opposition to the passage of an electric current through that conductor."@en ;
        rdfs:label       "Electrical Resistance"@en ;
        rdfs:subClassOf  qu:QuantityKind .

m3-lite:Shower  a        owl:Class ;
        rdfs:comment     "An actuator to automatically switch on/off the shower."@en ;
        rdfs:label       "Shower"@en ;
        rdfs:subClassOf  iot-lite:ActuatingDevice ;
        rdfs:subClassOf  [ a                   owl:Restriction ;
                           owl:onProperty      m3-lite:domainOfInterest ;
                           owl:someValuesFrom  m3-lite:BuildingAutomation
                         ] .

m3-lite:Hertz  a         owl:Class ;
        rdfs:comment     "Hertz"@en ;
        rdfs:label       "Hertz"@en ;
        rdfs:subClassOf  qu:Unit .

m3-lite:GPSSensor  a     owl:Class ;
        rdfs:comment     "Used in iPhone4 which allows the phone to localize itself."@en ;
        rdfs:label       "GPS Sensor"@en ;
        rdfs:subClassOf  ssn:SensingDevice ;
        rdfs:subClassOf  [ a                   owl:Restriction ;
                           owl:onProperty      m3-lite:domainOfInterest ;
                           owl:someValuesFrom  m3-lite:Transportation
                         ] ;
        txn:hasImage     <http://sensormeasurement.appspot.com/images/sensor/gps.png> .

m3-lite:Ventilation  a   owl:Class ;
        rdfs:comment     "An actuator to automatically open/close the ventilation."@en ;
        rdfs:label       "Ventilation"@en ;
        rdfs:subClassOf  iot-lite:ActuatingDevice ;
        rdfs:subClassOf  [ a                   owl:Restriction ;
                           owl:onProperty      m3-lite:domainOfInterest ;
                           owl:someValuesFrom  m3-lite:BuildingAutomation
                         ] .

m3-lite:EnergyMeter  a   owl:Class ;
        rdfs:comment     "Sensor to measure energy"@en ;
        rdfs:label       "Energy Meter"@en ;
        rdfs:subClassOf  ssn:SensingDevice ;
        rdfs:subClassOf  [ a                   owl:Restriction ;
                           owl:onProperty      m3-lite:domainOfInterest ;
                           owl:someValuesFrom  m3-lite:EnergyFOI
                         ] .

m3-lite:RevolutionsPerMinute
        a                owl:Class ;
        rdfs:comment     "Revolutions per minute (abbreviated rpm, RPM, rev/min, r/min) is a measure of the frequency of rotation, specifically the number of rotations around a fixed axis in one minute. It is used as a measure of rotational speed of a mechanical component." ;
        rdfs:label       "Revolutions Per Minute"@en ;
        rdfs:subClassOf  qu:Unit .

m3-lite:SnowChains  a    owl:Class ;
        rdfs:comment     "The actuator Snow chains (on/off)"@en ;
        rdfs:label       "Snow Chains"@en ;
        rdfs:subClassOf  iot-lite:ActuatingDevice ;
        rdfs:subClassOf  [ a                   owl:Restriction ;
                           owl:onProperty      m3-lite:domainOfInterest ;
                           owl:someValuesFrom  m3-lite:Transportation
                         ] ;
        txn:hasImage     <http://sensormeasurement.appspot.com/images/sensor/snowChain.png> .

m3-lite:PresenceStateDriverCard
        a                owl:Class ;
        rdfs:label       "Presence State Driver Card"@en ;
        rdfs:subClassOf  m3-lite:PresenceState .

m3-lite:Second_time  a   owl:Class ;
        rdfs:comment     ""@en ;
        rdfs:label       "Second time"@en ;
        rdfs:subClassOf  qu:Unit .

m3-lite:PresenceStateDriverCard2
        a                owl:Class ;
        rdfs:comment     "Indicates the presence of the second driver card." ;
        rdfs:label       "Presence State Driver Card 2"@en ;
        rdfs:subClassOf  m3-lite:PresenceStateDriverCard .

m3-lite:Position  a      owl:Class ;
        rdfs:label       "Position"@en ;
        rdfs:subClassOf  qu:QuantityKind .

m3-lite:TrackingParkingSpace
        a                owl:Class ;
        rdfs:comment     ""@en ;
        rdfs:label       "Tracking ParkingSpace"@en ;
        rdfs:subClassOf  m3-lite:TrackingGood .

m3-lite:Oxygen_Sensor
        a                owl:Class ;
        rdfs:comment     "Oxygen Sensor"@en ;
        rdfs:label       "Oxygen Sensor"@en ;
        rdfs:subClassOf  m3-lite:GaseousPollutantSensor .

m3-lite:AccelerationInstantaneous
        a                owl:Class ;
        rdfs:label       "Acceleration Instantaneous" ;
        rdfs:subClassOf  m3-lite:Acceleration .

m3-lite:WindDirectionSensor
        a                owl:Class ;
        rdfs:comment     "Wind Direction Sensor, unit in Degree"@en ;
        rdfs:label       "Wind Direction Sensor"@en ;
        rdfs:subClassOf  ssn:SensingDevice ;
        rdfs:subClassOf  [ a                   owl:Restriction ;
                           owl:onProperty      m3-lite:domainOfInterest ;
                           owl:someValuesFrom  m3-lite:Weather
                         ] ;
        txn:hasImage     <http://sensormeasurement.appspot.com/images/sensor/windDirection.png> .

m3-lite:Inch  a          owl:Class ;
        rdfs:comment     ""@en ;
        rdfs:label       "Inch"@en ;
        rdfs:subClassOf  qu:Unit .

m3-lite:CD  a            owl:Class ;
        rdfs:comment     "An RFID tag is embedded on CD."@en ;
        rdfs:label       "CD"@en ;
        rdfs:seeAlso     mo:CD , dbpedia:Album ;
        rdfs:subClassOf  m3-lite:RFIDQuantityKind .

m3-lite:CO2  a           owl:Class ;
        rdfs:comment     "To measure air quality"@en ;
        rdfs:label       "CO2 measurements"@en ;
        rdfs:subClassOf  qu:QuantityKind .

m3-lite:FillLevelGasTank
        a                owl:Class ;
        rdfs:comment     "Ratio of volume of combustible exhaust fluid to the total volume of diesel exhaust fluid storage container." ;
        rdfs:label       "Fill Level Gas Tank"@en ;
        rdfs:subClassOf  m3-lite:FillLevel .

m3-lite:WorkingStateDriver
        a                owl:Class ;
        rdfs:label       "Working State Driver"@en ;
        rdfs:subClassOf  m3-lite:WorkingState .

m3-lite:TimeRelatedStateDriver2
        a                owl:Class ;
        rdfs:comment     "Indicates if the second driver approaches or exceeds working time limits (or other limits)." ;
        rdfs:label       "Time Related State Driver 2"@en ;
        rdfs:subClassOf  m3-lite:TimeRelatedStateDriver .

m3-lite:Kilo  a          owl:Class ;
        rdfs:label       "Kilo"@en ;
        rdfs:subClassOf  qu:Unit .

m3-lite:Kelvin  a        owl:Class ;
        rdfs:comment     "Kelvin is a unit of measurement for temperature."@en ;
        rdfs:label       "Kelvin, Degree Kelvin"@en ;
        rdfs:seeAlso     sweet_unit:kelvin ;
        rdfs:subClassOf  qu:Unit .

m3-lite:MillivoltPerMeter
        a                owl:Class ;
        rdfs:label       "MillivoltPerMeter, MillivoltPerMetre" ;
        rdfs:subClassOf  qu:Unit .

m3-lite:Pedometer  a     owl:Class ;
        rdfs:comment     "Pedometer is used to count the number of steps when walking, running, etc."@en ;
        rdfs:label       "Pedometer"@en ;
        rdfs:subClassOf  ssn:SensingDevice ;
        rdfs:subClassOf  [ a                   owl:Restriction ;
                           owl:onProperty      m3-lite:domainOfInterest ;
                           owl:someValuesFrom  m3-lite:Health
                         ] .

m3-lite:ECG  a           owl:Class ;
        rdfs:comment     "ECG or EKG (Electrocardiogram)"@en ;
        rdfs:label       "ECG or EKG (Electrocardiogram)"@en ;
        rdfs:subClassOf  ssn:SensingDevice ;
        rdfs:subClassOf  [ a                   owl:Restriction ;
                           owl:onProperty      m3-lite:domainOfInterest ;
                           owl:someValuesFrom  m3-lite:Health
                         ] ;
        rdfs:subClassOf  [ a                   owl:Restriction ;
                           owl:onProperty      m3-lite:domainOfInterest ;
                           owl:someValuesFrom  m3-lite:Emotion
                         ] .

m3-lite:VoltageSensor
        a                owl:Class ;
        rdfs:comment     "The Com4Innov testbed is providing voltage sensor."@en ;
        rdfs:label       "Voltage Sensor"@en ;
        rdfs:subClassOf  ssn:SensingDevice .

m3-lite:WattPerSquareMeter
        a                owl:Class ;
        rdfs:comment     "Unit to measure solar radiation"@en ;
        rdfs:label       "Watt Per Square Metre, Watt Per Square Meter"@en ;
        rdfs:seeAlso     "http://purl.oclc.org/NET/ssnx/qu/unit#wattPerSquareMetre" ;
        rdfs:subClassOf  qu:Unit .

m3-lite:WattPerMeterSquare
        a                owl:Class ;
        rdfs:label       "Watt Per Meter Square"@en ;
        rdfs:subClassOf  qu:Unit .

m3-lite:GramPerLiter  a  owl:Class ;
        rdfs:comment     ""@en ;
        rdfs:label       "GramPerLiter (g/L)"@en ;
        rdfs:subClassOf  qu:Unit .

m3-lite:Pascal  a        owl:Class ;
        rdfs:comment     "Unit for pressure (e.g., atmospheric pressure)"@en ;
        rdfs:label       "Pascal"@en ;
        rdfs:subClassOf  qu:Unit .

ssn:Device  a   owl:Class .

dc:title  a     owl:AnnotationProperty .

m3-lite:SPO2  a          owl:Class ;
        rdfs:comment     "SPO2 measurement"@en ;
        rdfs:label       "SPO2"@en ;
        rdfs:subClassOf  qu:QuantityKind .

m3-lite:Pressure  a      owl:Class ;
        rdfs:comment     ""@en ;
        rdfs:label       "Pressure"@en ;
        rdfs:seeAlso     <http://archive.knoesis.org/research/semsci/application_domain/sem_sensor/ont/sensor-observation.owlPressureProperty> ;
        rdfs:subClassOf  qu:QuantityKind .

m3-lite:MmolPerLiter  a  owl:Class ;
        rdfs:comment     "MmolPerLiter unit to measure cholesterol"@en ;
        rdfs:label       "MmolPerLiter"@en ;
        rdfs:subClassOf  qu:Unit .

m3-lite:DewPointSensor
        a                owl:Class ;
        rdfs:comment     "It is the temperature to which air must be cooled at constant pressure and water content to reach saturation. The Com4Innov testbed is providing dew point sensor."@en ;
        rdfs:label       "Dew Point Sensor"@en ;
        rdfs:subClassOf  ssn:SensingDevice .

m3-lite:Location  a      owl:Class ;
        rdfs:comment     ""@en ;
        rdfs:label       "Location"@en ;
        rdfs:seeAlso     wgs84_pos:SpatialThing ;
        rdfs:subClassOf  qu:QuantityKind .

m3-lite:Precipitation
        a                owl:Class ;
        rdfs:comment     "Precipitation or rainfall measurements"@en ;
        rdfs:label       "Precipitation"@en ;
        rdfs:seeAlso     shw:Precipitation , <http://archive.knoesis.org/research/semsci/application_domain/sem_sensor/ont/sensor-observation.owlPrecipitationProperty> ;
        rdfs:subClassOf  qu:QuantityKind .

m3-lite:Ampere  a        owl:Class ;
        rdfs:comment     "The ampere is the SI unit for measuring an electric current which is the flow of electric charges through a surface at the rate of one coulomb per second.The ampere is the SI unit for measuring an electric current which is the flow of electric charges through a surface at the rate of one coulomb per second."@en ;
        rdfs:label       "Ampere (A)"@en ;
        rdfs:seeAlso     "http://purl.oclc.org/NET/ssnx/qu/unit#ampere" ;
        rdfs:seeAlso     sweet_unit:ampere , qudt_unit:Ampere ;
        rdfs:subClassOf  qu:Unit .

m3-lite:Millivolt  a     owl:Class ;
        rdfs:label       "Millivolt (mV)" ;
        rdfs:subClassOf  m3-lite:Volt .

vs:term_status  a  owl:AnnotationProperty .

m3-lite:DegreeFahrenheit
        a                owl:Class ;
        rdfs:comment     ""@en ;
        rdfs:label       "Degree fahrenheit"@en ;
        rdfs:seeAlso     sweet_unit:degreeF , weather:fahrenheit ;
        rdfs:subClassOf  m3-lite:Degree .

m3-lite:Accelerometer
        a                owl:Class ;
        rdfs:comment     "Accelerometer, Motion detector/Sensor. In iPhone 4, accelerometers are used to automatically determine the orientation in which the user is holding the phone (portrait or landscape)."@en ;
        rdfs:label       "Accelerometer"@en ;
        rdfs:seeAlso     cose:Accelerometer ;
        rdfs:subClassOf  ssn:SensingDevice ;
        rdfs:subClassOf  [ a                   owl:Restriction ;
                           owl:onProperty      m3-lite:domainOfInterest ;
                           owl:someValuesFrom  m3-lite:Activity
                         ] ;
        rdfs:subClassOf  [ a                   owl:Restriction ;
                           owl:onProperty      m3-lite:domainOfInterest ;
                           owl:someValuesFrom  m3-lite:Transportation
                         ] .

m3-lite:PPM  a           owl:Class ;
        rdfs:comment     "Used by CO2 sensor level"@en ;
        rdfs:label       "PPM (parts per million)"@en ;
        rdfs:subClassOf  qu:Unit .

m3-lite:FillLevelGasTank1
        a                owl:Class ;
        rdfs:comment     "Ratio of volume of combustible exhaust fluid to the total volume of diesel exhaust fluid storage container. This is the value for the primary tank of the vehicle." ;
        rdfs:label       "Fill Level Gas Tank 1"@en ;
        rdfs:subClassOf  m3-lite:FillLevelGasTank .

m3-lite:LitrePer100Kilometres
        a                owl:Class ;
        rdfs:comment     "A consumption unit which is equal to the one of a vehicle which needs 1 fuel litre in order to traverse 100 kilometres." ;
        rdfs:label       "LitrePer100Kilometres, LiterPer100Kilometers" ;
        rdfs:subClassOf  qu:Unit .

m3-lite:Fire  a          owl:Class ;
        rdfs:comment     ""@en ;
        rdfs:label       "Fire"@en ;
        rdfs:subClassOf  m3-lite:Environment .

m3-lite:Lamp  a          owl:Class ;
        rdfs:comment     "An actuator to automatically switch on/off the lamp."@en ;
        rdfs:label       "Lamp Actuator"@en ;
        rdfs:subClassOf  iot-lite:ActuatingDevice ;
        rdfs:subClassOf  [ a                   owl:Restriction ;
                           owl:onProperty      m3-lite:domainOfInterest ;
                           owl:someValuesFrom  m3-lite:BuildingAutomation
                         ] .

m3-lite:TrackingFood  a  owl:Class ;
        rdfs:comment     ""@en ;
        rdfs:label       "Tracking Food"@en ;
        rdfs:subClassOf  m3-lite:TrackingGood .

m3-lite:TrackingBook  a  owl:Class ;
        rdfs:comment     ""@en ;
        rdfs:label       "Tracking Book"@en ;
        rdfs:subClassOf  m3-lite:TrackingGood .

m3-lite:RelativeHumidity
        a                owl:Class ;
        rdfs:comment     "The ratio of vapour pressure to saturation vapour pressure, where vapour pressure is the pressure exerted by the molecules of water vapour and saturation vapour pressure is the pressure exerted by molecules of water vapour in AIR that has attained saturation." ;
        rdfs:label       "Relative Humidity"@en ;
        rdfs:seeAlso     "http://sweet.jpl.nasa.gov/ontology/property.owl#RelativeHumidity" ;
        rdfs:subClassOf  qu:QuantityKind .

m3-lite:BloodPressureSensor
        a                owl:Class ;
        rdfs:comment     "Blood Pressure Sensor"@en ;
        rdfs:label       "Blood Pressure Sensor"@en ;
        rdfs:subClassOf  ssn:SensingDevice ;
        rdfs:subClassOf  [ a                   owl:Restriction ;
                           owl:onProperty      m3-lite:domainOfInterest ;
                           owl:someValuesFrom  m3-lite:Health
                         ] ;
        txn:hasImage     <http://sensormeasurement.appspot.com/images/sensor/bloodPressure.png> .

m3-lite:Candela  a       owl:Class ;
        rdfs:comment     ""@en ;
        rdfs:label       "Candela"@en ;
        rdfs:seeAlso     sweet_unit:candela ;
        rdfs:subClassOf  qu:Unit .

m3-lite:Frequency  a     owl:Class ;
        rdfs:comment     "Frequency"@en ;
        rdfs:label       "Frequency"@en ;
        rdfs:subClassOf  qu:QuantityKind .

m3-lite:SpeedAverage  a  owl:Class ;
        rdfs:comment     "A measure of the average rate of motion of an object." ;
        rdfs:label       "Speed Average"@en ;
        rdfs:subClassOf  m3-lite:Speed .

m3-lite:VehicleOverspeedState
        a                owl:Class ;
        rdfs:comment     "Indicates whether the vehicle is exceeding the legal speed limit." ;
        rdfs:label       "Vehicle Overspeed State"@en ;
        rdfs:subClassOf  qu:QuantityKind .

m3-lite:QRCode  a        owl:Class ;
        rdfs:comment     "A tagging device can be QRCode"@en ;
        rdfs:label       "QRCode"@en ;
        rdfs:subClassOf  iot-lite:TagDevice .

m3-lite:TrafficCongestion
        a                owl:Class ;
        rdfs:comment     "Descriptive level of road traffic congestion within a defined area." ;
        rdfs:label       "Traffic Congestion"@en ;
        rdfs:subClassOf  qu:QuantityKind .

m3-lite:KiloWattHour  a  owl:Class ;
        rdfs:comment     "Unit to measure electricity by electricity meter devicesy"@en ;
        rdfs:label       "Kilo Watt Hour"@en ;
        rdfs:seeAlso     qudt_unit:KiloWatthour ;
        rdfs:subClassOf  qu:Unit .

m3-lite:MagneticField
        a                owl:Class ;
        rdfs:comment     "Magnetic Field"@en ;
        rdfs:label       "Magnetic Field"@en ;
        rdfs:subClassOf  qu:QuantityKind .

m3-lite:CloudCover  a    owl:Class ;
        rdfs:comment     "Cloud Cover"@en ;
        rdfs:label       "Cloud Cover"@en ;
        rdfs:subClassOf  qu:QuantityKind .

m3-lite:AlarmSystem  a   owl:Class ;
        rdfs:comment     "An actuator to automatically switch on/off the alarm system."@en ;
        rdfs:label       "Alarm Systemr"@en ;
        rdfs:subClassOf  iot-lite:ActuatingDevice ;
        rdfs:subClassOf  [ a                   owl:Restriction ;
                           owl:onProperty      m3-lite:domainOfInterest ;
                           owl:someValuesFrom  m3-lite:Transportation
                         ] ;
        rdfs:subClassOf  [ a                   owl:Restriction ;
                           owl:onProperty      m3-lite:domainOfInterest ;
                           owl:someValuesFrom  m3-lite:BuildingAutomation
                         ] .

m3-lite:FillLevelWasteContainer
        a                owl:Class ;
        rdfs:label       "Fill Level Waste Container"@en ;
        rdfs:subClassOf  m3-lite:FillLevel ;
        dc:description   "Ratio between the current filleage level and the total capacity of a waste container." .

m3-lite:UltrasonicSensor
        a                owl:Class ;
        rdfs:comment     "Ultrasonic sensors are used to deduce human posture in smart home for example."@en ;
        rdfs:label       "Ultrasonic Sensor"@en ;
        rdfs:subClassOf  ssn:SensingDevice ;
        rdfs:subClassOf  [ a                   owl:Restriction ;
                           owl:onProperty      m3-lite:domainOfInterest ;
                           owl:someValuesFrom  m3-lite:BuildingAutomation
                         ] .

m3-lite:Window  a        owl:Class ;
        rdfs:comment     "An actuator to automatically open/close the window."@en ;
        rdfs:label       "Window"@en ;
        rdfs:subClassOf  iot-lite:ActuatingDevice ;
        rdfs:subClassOf  [ a                   owl:Restriction ;
                           owl:onProperty      m3-lite:domainOfInterest ;
                           owl:someValuesFrom  m3-lite:BuildingAutomation
                         ] .

m3-lite:Liter  a         owl:Class ;
        rdfs:comment     "A metric unit of capacity defined as the volume of one kilogram of water under standard conditions. It is equal to 1,000 cubic centimetres."@en ;
        rdfs:label       "Liter, Litre"@en ;
        rdfs:seeAlso     "http://purl.oclc.org/NET/ssnx/qu/unit#litre" ;
        rdfs:subClassOf  qu:Unit .

m3-lite:AlcoholLevel  a  owl:Class ;
        rdfs:comment     "Alcohol Level"@en ;
        rdfs:label       "Alcohol Level"@en ;
        rdfs:subClassOf  qu:QuantityKind .

m3-lite:Glucometer  a    owl:Class ;
        rdfs:comment     "Glucometer, Blood sugar, blood glucose level"@en ;
        rdfs:label       "Glucometer"@en ;
        rdfs:subClassOf  ssn:SensingDevice ;
        rdfs:subClassOf  [ a                   owl:Restriction ;
                           owl:onProperty      m3-lite:domainOfInterest ;
                           owl:someValuesFrom  m3-lite:Health
                         ] ;
        txn:hasImage     <http://sensormeasurement.appspot.com/images/sensor/glucometer.png> .

m3-lite:Place  a         owl:Class ;
        rdfs:comment     "Location, Place, GPS coordinates as an Internet of Things (IoT) applicative domain."@en ;
        rdfs:label       "Location"@en ;
        rdfs:subClassOf  m3-lite:DomainOfInterest .

m3-lite:Milliwatt  a     owl:Class ;
        rdfs:label       "Milliwatt (mW)" ;
        rdfs:subClassOf  m3-lite:Watt .

m3-lite:MeterPerSecondSquare
        a                owl:Class ;
        rdfs:label       "MeterPerSecondSquare)"@en ;
        rdfs:seeAlso     <http://purl.oclc.org/NET/ssnx/qu/unit#metrePerSecondSquared> ;
        rdfs:subClassOf  qu:Unit .

m3-lite:FuelConsumption
        a                owl:Class ;
        rdfs:label       "Fuel Consumption"@en ;
        rdfs:subClassOf  qu:QuantityKind .

qudt_unit:Bar  a         owl:Class ;
        rdfs:comment     "Metric unit of atmospheric pressure equal to 14.50 pounds per square inch (lb/in2), 1.02 kilograms per square centimeter (kg/cm2), 29.53 inches of mercury (in Hg), or 0.9869 atmosphere."@en ;
        rdfs:label       "Bar"@en ;
        rdfs:seeAlso     "http://qudt.org/vocab/unit#Bar" ;
        rdfs:subClassOf  qu:Unit .

m3-lite:SeatBeltTensionSensor
        a                owl:Class ;
        rdfs:comment     ""@en ;
        rdfs:label       "Seat belt tension actuator (on/off)"@en ;
        rdfs:subClassOf  iot-lite:ActuatingDevice ;
        rdfs:subClassOf  [ a                   owl:Restriction ;
                           owl:onProperty      m3-lite:domainOfInterest ;
                           owl:someValuesFrom  m3-lite:Transportation
                         ] ;
        txn:hasImage     <http://sensormeasurement.appspot.com/images/sensor/seatBelt.png> .

m3-lite:WorkingStateDriver1
        a                owl:Class ;
        rdfs:comment     "State of work of the first driver as defined in the FMS standard." ;
        rdfs:label       "Working State Driver 1"@en ;
        rdfs:subClassOf  m3-lite:WorkingStateDriver .

m3-lite:BatteryLevel  a  owl:Class ;
        rdfs:comment     "This property holds the percentage of the battery capacity that remains available."@en ;
        rdfs:label       "Battery level"@en ;
        rdfs:seeAlso     "http://www.w3.org/2007/uwa/context/deliveryContext.owl#BatteryLevel" ;
        rdfs:subClassOf  qu:QuantityKind .

m3-lite:Microvolt  a     owl:Class ;
        rdfs:label       "Microvolt (uV)" ;
        rdfs:subClassOf  m3-lite:Volt .

m3-lite:Speed  a         owl:Class ;
        rdfs:comment     ""@en ;
        rdfs:label       "Speed"@en ;
        rdfs:seeAlso     "http://purl.oclc.org/NET/ssnx/qu/quantity#speed" ;
        rdfs:subClassOf  qu:QuantityKind .

m3-lite:VehicleCountSensor
        a                owl:Class ;
        rdfs:comment     "To count the number of vehicles (e.g., used within the Citypulse project)"@en ;
        rdfs:label       "Vehicle Count Sensor"@en ;
        rdfs:subClassOf  ssn:SensingDevice ;
        rdfs:subClassOf  [ a                   owl:Restriction ;
                           owl:onProperty      m3-lite:domainOfInterest ;
                           owl:someValuesFrom  m3-lite:Transportation
                         ] .

m3-lite:Lux  a           owl:Class ;
        rdfs:comment     "The SI unit of illuminance, equal to one lumen per square metre."@en ;
        rdfs:label       "Lux (lx)"@en ;
        rdfs:seeAlso     "http://purl.oclc.org/NET/ssnx/qu/unit#lux" ;
        rdfs:seeAlso     sweet_unit:lux , qudt_unit:Lux ;
        rdfs:subClassOf  qu:Unit .

m3-lite:MotionState  a   owl:Class ;
        rdfs:label       "Motion State"@en ;
        rdfs:subClassOf  qu:QuantityKind .

m3-lite:DirectionHeading
        a                owl:Class ;
        rdfs:comment     "The course or direction in which a object (vehicle, person, ...) is pointing or moving." ;
        rdfs:label       "Direction Heading"@en ;
        rdfs:subClassOf  m3-lite:Direction .

m3-lite:Lumen  a         owl:Class ;
        rdfs:comment     "The SI unit of luminous flux, equal to the amount of light emitted per second in a unit solid angle of one steradian from a uniform source of one candela."@en ;
        rdfs:label       "Lumen (lm)"@en ;
        rdfs:seeAlso     "http://purl.oclc.org/NET/ssnx/qu/unit#lumen" ;
        rdfs:subClassOf  qu:Unit .

m3-lite:GramPerCubicMetre
        a                owl:Class ;
        rdfs:subClassOf  qu:Unit .

m3-lite:Millimetre  a    owl:Class ;
        rdfs:label       "Millimetre, millimeter" ;
        rdfs:subClassOf  m3-lite:Meter .

m3-lite:Pound  a         owl:Class ;
        rdfs:comment     ""@en ;
        rdfs:label       "Pound"@en ;
        rdfs:subClassOf  qu:Unit .

m3-lite:MileageTotal  a  owl:Class ;
        rdfs:comment     "The total distance travelled by the particular vehicle since its initial production." ;
        rdfs:label       "Mileage Total"@en ;
        rdfs:subClassOf  m3-lite:Mileage .

m3-lite:SpeedSensor  a   owl:Class ;
        rdfs:comment     "Car Speed Sensor, speedometer or Velocity used in a car"@en ;
        rdfs:label       "Car Speed Sensor"@en ;
        rdfs:subClassOf  ssn:SensingDevice ;
        rdfs:subClassOf  [ a                   owl:Restriction ;
                           owl:onProperty      m3-lite:domainOfInterest ;
                           owl:someValuesFrom  m3-lite:Transportation
                         ] ;
        txn:hasImage     <http://sensormeasurement.appspot.com/images/sensor/speed.png> .

m3-lite:WeatherPrecipitation
        a                owl:Class ;
        rdfs:comment     ""@en ;
        rdfs:label       "Weather Precipitation"@en ;
        rdfs:subClassOf  m3-lite:Precipitation .

m3-lite:Curtain  a       owl:Class ;
        rdfs:comment     "An actuator to automatically open/close the curtain."@en ;
        rdfs:label       "Curtain"@en ;
        rdfs:subClassOf  iot-lite:ActuatingDevice ;
        rdfs:subClassOf  [ a                   owl:Restriction ;
                           owl:onProperty      m3-lite:domainOfInterest ;
                           owl:someValuesFrom  m3-lite:BuildingAutomation
                         ] .

m3-lite:RoadSurfaceThermometer
        a                owl:Class ;
        rdfs:comment     "Road Surface Thermometer"@en ;
        rdfs:label       "Road Surface Thermometer"@en ;
        rdfs:subClassOf  ssn:SensingDevice ;
        rdfs:subClassOf  [ a                   owl:Restriction ;
                           owl:onProperty      m3-lite:domainOfInterest ;
                           owl:someValuesFrom  m3-lite:Transportation
                         ] ;
        txn:hasImage     <http://sensormeasurement.appspot.com/images/sensor/thermometer.png> .

m3-lite:Event  a         owl:Class ;
        rdfs:comment     ""@en ;
        rdfs:label       "Event"@en ;
        rdfs:subClassOf  m3-lite:Place .

m3-lite:EnergyFOI  a     owl:Class ;
        rdfs:comment     "Energy or Smart Grid as an Internet of Things (IoT) applicative domain."@en ;
        rdfs:label       "Energy"@en ;
        rdfs:subClassOf  m3-lite:DomainOfInterest .

m3-lite:Kilometre  a     owl:Class ;
        rdfs:label       "Kilometre, Kilometer" ;
        rdfs:subClassOf  m3-lite:Meter .

m3-lite:LightSensor  a   owl:Class ;
        rdfs:comment     "Light/Illuminance Sensor is used in iPhone4 to adjust the brightness of the screen."@en ;
        rdfs:label       "Light Sensor"@en ;
        rdfs:subClassOf  ssn:SensingDevice ;
        rdfs:subClassOf  [ a                   owl:Restriction ;
                           owl:onProperty      m3-lite:domainOfInterest ;
                           owl:someValuesFrom  m3-lite:BuildingAutomation
                         ] ;
        rdfs:subClassOf  [ a                   owl:Restriction ;
                           owl:onProperty      m3-lite:domainOfInterest ;
                           owl:someValuesFrom  m3-lite:Transportation
                         ] ;
        rdfs:subClassOf  [ a                   owl:Restriction ;
                           owl:onProperty      m3-lite:domainOfInterest ;
                           owl:someValuesFrom  m3-lite:Weather
                         ] ;
        txn:hasImage     <http://sensormeasurement.appspot.com/images/sensor/light.png> .

m3-lite:Gram  a          owl:Class ;
        rdfs:label       "Gram (g)" ;
        rdfs:subClassOf  qu:Unit .

m3-lite:TrackingToll  a  owl:Class ;
        rdfs:comment     ""@en ;
        rdfs:label       "Tracking Toll"@en ;
        rdfs:subClassOf  m3-lite:TrackingGood .

m3-lite:Centibar  a      owl:Class ;
        rdfs:comment     "The centibar is a unit of pressure defined as 1e-2 bar." ;
        rdfs:label       "Centibar"@en ;
        rdfs:subClassOf  qudt_unit:Bar .

m3-lite:EAQI  a          owl:Class ;
        rdfs:comment     ""@en ;
        rdfs:label       "European Air Quality Index (EAQI)"@en ;
        rdfs:subClassOf  qu:Unit .

m3-lite:Monument  a      owl:Class ;
        rdfs:comment     ""@en ;
        rdfs:label       "Monument"@en ;
        rdfs:subClassOf  m3-lite:Place .

m3-lite:ABS  a           owl:Class ;
        rdfs:comment     "The actuator ABS (on/off)"@en ;
        rdfs:label       "ABS (Anti-lock braking system)"@en ;
        rdfs:subClassOf  iot-lite:ActuatingDevice ;
        rdfs:subClassOf  [ a                   owl:Restriction ;
                           owl:onProperty      m3-lite:domainOfInterest ;
                           owl:someValuesFrom  m3-lite:Transportation
                         ] ;
        txn:hasImage     <http://sensormeasurement.appspot.com/images/sensor/abs.png> .

m3-lite:FillLevelGasTank2
        a                owl:Class ;
        rdfs:comment     "Ratio of volume of combustible exhaust fluid to the total volume of diesel exhaust fluid storage container. This is the value for the secondary tank of the vehicle." ;
        rdfs:label       "Fill Level Gas Tank 2"@en ;
        rdfs:subClassOf  m3-lite:FillLevelGasTank .

m3-lite:Microwatt  a     owl:Class ;
        rdfs:label       "Microwatt (uW)" ;
        rdfs:subClassOf  m3-lite:Watt .

m3-lite:ReactivePower
        a                owl:Class ;
        rdfs:comment     "The portion of electricity that establishes and sustains the electric and magnetic fields of alternating-current equipment." ;
        rdfs:label       "Reactive Power"@en ;
        rdfs:seeAlso     "http://purl.oclc.org/NET/ssnx/qu/dim#ReactivePower" ;
        rdfs:subClassOf  m3-lite:Power .

m3-lite:Motion  a        owl:Class ;
        rdfs:comment     ""@en ;
        rdfs:label       "Motion"@en ;
        rdfs:seeAlso     spitfire:Motion ;
        rdfs:subClassOf  qu:QuantityKind .

m3-lite:DistanceSensor
        a                owl:Class ;
        rdfs:comment     "Distance Sensor to detect the safety distance with other cars for instance (it can be a laser)."@en ;
        rdfs:label       "Distance Sensor"@en ;
        rdfs:subClassOf  ssn:SensingDevice ;
        rdfs:subClassOf  [ a                   owl:Restriction ;
                           owl:onProperty      m3-lite:domainOfInterest ;
                           owl:someValuesFrom  m3-lite:Transportation
                         ] ;
        txn:hasImage     <http://sensormeasurement.appspot.com/images/sensor/distance.png> .

m3-lite:VehiclesPerMinute
        a                owl:Class ;
        rdfs:comment     "Number of vehicles that traverse a concrete region of the space in one minute." ;
        rdfs:label       "Vehicles Per Minute"@en ;
        rdfs:subClassOf  qu:Unit .

m3-lite:AirConditioner
        a                owl:Class ;
        rdfs:comment     "An actuator to automatically switch on/off the air conditioner."@en ;
        rdfs:label       "Air conditioner"@en ;
        rdfs:subClassOf  iot-lite:ActuatingDevice ;
        rdfs:subClassOf  [ a                   owl:Restriction ;
                           owl:onProperty      m3-lite:domainOfInterest ;
                           owl:someValuesFrom  m3-lite:Transportation
                         ] ;
        rdfs:subClassOf  [ a                   owl:Restriction ;
                           owl:onProperty      m3-lite:domainOfInterest ;
                           owl:someValuesFrom  m3-lite:BuildingAutomation
                         ] .

m3-lite:Ohm  a           owl:Class ;
        rdfs:comment     "Ohm is the unit of electrical resistance."@en ;
        rdfs:label       "Ohm"@en ;
        rdfs:seeAlso     sweet_unit:ohm ;
        rdfs:subClassOf  qu:Unit .

m3-lite:Calcium  a       owl:Class ;
        rdfs:comment     "Blood Calcium level"@en ;
        rdfs:label       "Calcium"@en ;
        rdfs:subClassOf  qu:QuantityKind .

m3-lite:Door  a          owl:Class ;
        rdfs:comment     "An actuator to automatically open/close the door."@en ;
        rdfs:label       "Door"@en ;
        rdfs:subClassOf  iot-lite:ActuatingDevice ;
        rdfs:subClassOf  [ a                   owl:Restriction ;
                           owl:onProperty      m3-lite:domainOfInterest ;
                           owl:someValuesFrom  m3-lite:BuildingAutomation
                         ] .

m3-lite:BuildingTemperature
        a                owl:Class ;
        rdfs:comment     ""@en ;
        rdfs:label       "Building/Room Temperature"@en ;
        rdfs:subClassOf  m3-lite:Temperature .

m3-lite:SoundPressureLevelAmbient
        a                owl:Class ;
        rdfs:label       "Sound Pressure Level Ambient"@en ;
        rdfs:subClassOf  m3-lite:SoundPressureLevel .

m3-lite:Weather  a       owl:Class ;
        rdfs:comment     "Weather Forecasting, Meterology as an Internet of Things (IoT) applicative domain."@en ;
        rdfs:label       "Weather Forecasting"@en ;
        rdfs:seeAlso     <http://archive.knoesis.org/research/semsci/application_domain/sem_sensor/ont/sensor-observation.owlWeatherObservation> ;
        rdfs:subClassOf  m3-lite:DomainOfInterest .

m3-lite:NO_Sensor  a     owl:Class ;
        rdfs:comment     "Nitrogen Oxide (NO) Sensor"@en ;
        rdfs:label       "Nitrogen Oxide (NO) Sensor"@en ;
        rdfs:subClassOf  m3-lite:GaseousPollutantSensor .

m3-lite:ESP  a           owl:Class ;
        rdfs:comment     "The actuator ESP (on/off)"@en ;
        rdfs:label       "ESP (Electronic Stability Program)"@en ;
        rdfs:subClassOf  iot-lite:ActuatingDevice ;
        rdfs:subClassOf  [ a                   owl:Restriction ;
                           owl:onProperty      m3-lite:domainOfInterest ;
                           owl:someValuesFrom  m3-lite:Transportation
                         ] ;
        txn:hasImage     <http://sensormeasurement.appspot.com/images/sensor/esp.png> .

m3-lite:ChemicalAgentAtmosphericConcentration
        a                owl:Class ;
        rdfs:label       "Chemical Agent Atmospheric Concentration" ;
        rdfs:subClassOf  qu:QuantityKind .

m3-lite:FuelLevel  a     owl:Class ;
        rdfs:comment     "Fuel Level Sensor is used in car."@en ;
        rdfs:label       "Fuel Level Sensor"@en ;
        rdfs:subClassOf  ssn:SensingDevice ;
        rdfs:subClassOf  [ a                   owl:Restriction ;
                           owl:onProperty      m3-lite:domainOfInterest ;
                           owl:someValuesFrom  m3-lite:Transportation
                         ] ;
        txn:hasImage     <http://sensormeasurement.appspot.com/images/sensor/fuel.png> .

m3-lite:ElectricField900Mhz
        a                owl:Class ;
        rdfs:comment     "A field of force associated with a moving electric charge equivalent to an electric field and a magnetic field at right angles to each other and to the direction of propagation. Applied to the 900 MHz UHF band." ;
        rdfs:label       "Electric Field 900 MHz"@en ;
        rdfs:subClassOf  m3-lite:ElectricField .

m3-lite:Kilogram  a      owl:Class ;
        rdfs:comment     "The SI unit of mass, it is equal to the mass of the international prototype of the kilogram."@en ;
        rdfs:label       "Kilogram (kg)"@en ;
        rdfs:seeAlso     "http://purl.oclc.org/NET/ssnx/qu/unit#kilogram" ;
        rdfs:subClassOf  m3-lite:Gram .

m3-lite:WindDirection
        a                owl:Class ;
        rdfs:comment     "The geodetic azimuth of the direction from which the wind is blowing."@en ;
        rdfs:label       "Wind Direction"@en ;
        rdfs:seeAlso     shw:DirectionalWind ;
        rdfs:subClassOf  qu:QuantityKind .

m3-lite:AirPollutantSensor
        a                owl:Class ;
        rdfs:comment     "Air Pollutant Sensor"@en ;
        rdfs:label       "Air Pollutant Sensor"@en ;
        rdfs:subClassOf  ssn:SensingDevice ;
        rdfs:subClassOf  [ a                   owl:Restriction ;
                           owl:onProperty      m3-lite:domainOfInterest ;
                           owl:someValuesFrom  m3-lite:Environment
                         ] .

m3-lite:WeightSensor  a  owl:Class ;
        rdfs:comment     "Weight Sensor can be used to weigh a person."@en ;
        rdfs:label       "Weight Sensor"@en ;
        rdfs:subClassOf  ssn:SensingDevice ;
        rdfs:subClassOf  [ a                   owl:Restriction ;
                           owl:onProperty      m3-lite:domainOfInterest ;
                           owl:someValuesFrom  m3-lite:Health
                         ] ;
        txn:hasImage     <http://sensormeasurement.appspot.com/images/sensor/weight.png> .

m3-lite:Fridge  a        owl:Class ;
        rdfs:comment     "An actuator to automatically switch on/off the fridge."@en ;
        rdfs:label       "Fridge, refrigerator"@en ;
        rdfs:subClassOf  iot-lite:ActuatingDevice ;
        rdfs:subClassOf  [ a                   owl:Restriction ;
                           owl:onProperty      m3-lite:domainOfInterest ;
                           owl:someValuesFrom  m3-lite:BuildingAutomation
                         ] .

m3-lite:CoffeeMachine
        a                owl:Class ;
        rdfs:comment     "An actuator to automatically switch on/off the coffe machine."@en ;
        rdfs:label       "Coffee Machine, Coffee maker"@en ;
        rdfs:subClassOf  iot-lite:ActuatingDevice ;
        rdfs:subClassOf  [ a                   owl:Restriction ;
                           owl:onProperty      m3-lite:domainOfInterest ;
                           owl:someValuesFrom  m3-lite:BuildingAutomation
                         ] .

m3-lite:ThrottleSensor
        a                owl:Class ;
        rdfs:comment     "Throttle Position Sensor is used in cars."@en ;
        rdfs:label       "Throttle Position Sensor"@en ;
        rdfs:subClassOf  ssn:SensingDevice ;
        rdfs:subClassOf  [ a                   owl:Restriction ;
                           owl:onProperty      m3-lite:domainOfInterest ;
                           owl:someValuesFrom  m3-lite:Transportation
                         ] ;
        txn:hasImage     <http://sensormeasurement.appspot.com/images/sensor/throttle.png> .

m3-lite:Timestamp  a     owl:Class ;
        rdfs:comment     "Sequence of characters or encoded information identifying when a certain event occurred, usually giving date and time of day, sometimes accurate to a small fraction of a second. This representation should be encoded following ISO8601." ;
        rdfs:label       "Timestamp"@en ;
        rdfs:seeAlso     "http://sweet.jpl.nasa.gov/2.3/propTime.owl#Timestamp" ;
        rdfs:subClassOf  qu:QuantityKind .

m3-lite:Acceleration  a  owl:Class ;
        rdfs:comment     "The rate of change with time of the velocity vector of a particle." ;
        rdfs:seeAlso     "http://purl.oclc.org/NET/ssnx/qu/dim#Acceleration" ;
        rdfs:subClassOf  qu:QuantityKind .

m3-lite:Miles  a         owl:Class ;
        rdfs:comment     ""@en ;
        rdfs:label       "Miles"@en ;
        rdfs:subClassOf  qu:Unit .

m3-lite:WindSpeedSensor
        a                owl:Class ;
        rdfs:comment     "Wind Speed Sensor, Anemometer or Wind Velocity Sensor is used to measure the wind speed."@en ;
        rdfs:label       "Wind Speed Sensor"@en ;
        rdfs:subClassOf  ssn:SensingDevice ;
        rdfs:subClassOf  [ a                   owl:Restriction ;
                           owl:onProperty      m3-lite:domainOfInterest ;
                           owl:someValuesFrom  m3-lite:Environment
                         ] ;
        rdfs:subClassOf  [ a                   owl:Restriction ;
                           owl:onProperty      m3-lite:domainOfInterest ;
                           owl:someValuesFrom  m3-lite:Agriculture
                         ] ;
        rdfs:subClassOf  [ a                   owl:Restriction ;
                           owl:onProperty      m3-lite:domainOfInterest ;
                           owl:someValuesFrom  m3-lite:Weather
                         ] ;
        txn:hasImage     <http://sensormeasurement.appspot.com/images/sensor/wind.png> .

m3-lite:TrackingDVD  a   owl:Class ;
        rdfs:comment     ""@en ;
        rdfs:label       "Tracking DVD"@en ;
        rdfs:subClassOf  m3-lite:TrackingGood .

m3-lite:Farad  a         owl:Class ;
        rdfs:comment     ""@en ;
        rdfs:label       "Farad"@en ;
        rdfs:seeAlso     sweet_unit:farad ;
        rdfs:subClassOf  qu:Unit .

m3-lite:WaterLevel  a    owl:Class ;
        rdfs:comment     ""@en ;
        rdfs:label       "Water level"@en ;
        rdfs:subClassOf  qu:QuantityKind .

m3-lite:PresenceStatePeople
        a                owl:Class ;
        rdfs:comment     "The presence or absence of people passing." ;
        rdfs:label       "Presence State People"@en ;
        rdfs:subClassOf  m3-lite:PresenceState .

m3-lite:WorkingStateDriver2
        a                owl:Class ;
        rdfs:comment     "State of work of the second driver as defined in the FMS standard." ;
        rdfs:label       "Working State Driver 2"@en ;
        rdfs:subClassOf  m3-lite:WorkingStateDriver .

m3-lite:Restaurant  a    owl:Class ;
        rdfs:comment     ""@en ;
        rdfs:label       "Restaurant"@en ;
        rdfs:subClassOf  m3-lite:Place .

m3-lite:HeartBeat  a     owl:Class ;
        rdfs:comment     "HeartBeat, heart rate"@en ;
        rdfs:label       "Heartbeat"@en ;
        rdfs:subClassOf  qu:QuantityKind .

m3-lite:Lavatory  a      owl:Class ;
        rdfs:comment     "An actuator to automatically switch on/off the lavatory."@en ;
        rdfs:label       "Lavatory"@en ;
        rdfs:subClassOf  iot-lite:ActuatingDevice ;
        rdfs:subClassOf  [ a                   owl:Restriction ;
                           owl:onProperty      m3-lite:domainOfInterest ;
                           owl:someValuesFrom  m3-lite:BuildingAutomation
                         ] .

m3-lite:DewPoint  a      owl:Class ;
        rdfs:comment     "It is the temperature to which air must be cooled at constant pressure and water content to reach saturation. The Com4Innov testbed is providing dew point quantity kind. "@en ;
        rdfs:label       "Dew Point"@en ;
        rdfs:subClassOf  qu:QuantityKind .

m3-lite:Food  a          owl:Class ;
        rdfs:comment     "An RFID tag is embedded on food."@en ;
        rdfs:label       "Food"@en ;
        rdfs:seeAlso     naturopathy:Food , food_smart_product:FoodOrDrinkItem ;
        rdfs:subClassOf  m3-lite:RFIDQuantityKind .

m3-lite:AtmosphericPressureSensor
        a                owl:Class ;
        rdfs:comment     "Atmospheric Pressure Sensor, Barometer or Barometric Pressure Sensor is a scientific instrument used im meteorology to measure atmospheric pressure."@en ;
        rdfs:label       "Atmospheric Pressure Sensor"@en ;
        rdfs:seeAlso     aws:AtmosphericPressureSensor , cose:BarometricPressureSensor , weather:Pressure ;
        rdfs:subClassOf  ssn:SensingDevice ;
        rdfs:subClassOf  [ a                   owl:Restriction ;
                           owl:onProperty      m3-lite:domainOfInterest ;
                           owl:someValuesFrom  m3-lite:Agriculture
                         ] ;
        rdfs:subClassOf  [ a                   owl:Restriction ;
                           owl:onProperty      m3-lite:domainOfInterest ;
                           owl:someValuesFrom  m3-lite:Weather
                         ] .

m3-lite:PH  a            owl:Class ;
        rdfs:comment     "PH"@en ;
        rdfs:label       "PH"@en ;
        rdfs:subClassOf  qu:QuantityKind .

m3-lite:SoilHumidity  a  owl:Class ;
        rdfs:comment     "Soil Humidity"@en ;
        rdfs:label       "Soil Humidity"@en ;
        rdfs:subClassOf  qu:QuantityKind .

m3-lite:Book  a          owl:Class ;
        rdfs:comment     "An RFID tag is embedded on book."@en ;
        rdfs:label       "Book"@en ;
        rdfs:seeAlso     dbpedia:Book ;
        rdfs:subClassOf  m3-lite:RFIDQuantityKind .

m3-lite:DegreeCelsius
        a                owl:Class ;
        rdfs:comment     "A temperature unit which is equal to one kelvin degree. However, they have their zeros at different points. The centigrade scale has its zero at 273.15 K."@en ;
        rdfs:label       "Degree celsius"@en ;
        rdfs:seeAlso     "http://purl.oclc.org/NET/ssnx/qu/unit#degreeCelsius" ;
        rdfs:seeAlso     sweet_unit:degreeC , qudt_unit:DegreeCelsius ;
        rdfs:subClassOf  m3-lite:Degree .

m3-lite:Drawer  a        owl:Class ;
        rdfs:comment     "An actuator to automatically open/close the drawer."@en ;
        rdfs:label       "Drawer"@en ;
        rdfs:subClassOf  iot-lite:ActuatingDevice ;
        rdfs:subClassOf  [ a                   owl:Restriction ;
                           owl:onProperty      m3-lite:domainOfInterest ;
                           owl:someValuesFrom  m3-lite:BuildingAutomation
                         ] .

m3-lite:AirTemperature
        a                owl:Class ;
        rdfs:comment     "The temperature of the air that would be indicated by a thermometer exposed to the air at a location sheltered from direct solar radiation."@en ;
        rdfs:label       "Air Temperature, Weather Temperature, Ambient Temperature"@en ;
        rdfs:seeAlso     shw:Temperature , openIoT:AirTemperature ;
        rdfs:subClassOf  m3-lite:Temperature .

m3-lite:Presence  a      owl:Class ;
        rdfs:comment     "A person is in the room or not."@en ;
        rdfs:label       "Presence"@en ;
        rdfs:subClassOf  qu:QuantityKind .

m3-lite:Minute_angle  a  owl:Class ;
        rdfs:comment     ""@en ;
        rdfs:label       "Minute_angle"@en ;
        rdfs:subClassOf  qu:Unit .

m3-lite:RoomTemperature
        a                owl:Class ;
        rdfs:comment     ""@en ;
        rdfs:label       "Room Temperature"@en ;
        rdfs:seeAlso     home:RoomTemperature , dogont:TemperatureMeasurementMNotification ;
        rdfs:subClassOf  m3-lite:BuildingTemperature .

m3-lite:GaseousPollutantSensor
        a                owl:Class ;
        rdfs:comment     "Gaseous Pollutant Sensor"@en ;
        rdfs:label       "Gaseous Pollutant Sensor"@en ;
        rdfs:subClassOf  m3-lite:AirPollutantSensor .

m3-lite:DiastolicBloodPressure
        a                owl:Class ;
        rdfs:comment     ""@en ;
        rdfs:label       "Diastolic Blood pressure"@en ;
        rdfs:subClassOf  m3-lite:BloodPressure .

m3-lite:Coulomb  a       owl:Class ;
        rdfs:comment     ""@en ;
        rdfs:label       "Coulomb"@en ;
        rdfs:seeAlso     sweet_unit:coulomb ;
        rdfs:subClassOf  qu:Unit .

m3-lite:MotionStateVehicle
        a                owl:Class ;
        rdfs:comment     "Indicates whether motion of the vehicle is detected or not." ;
        rdfs:label       "Motion State Vehicle"@en ;
        rdfs:subClassOf  m3-lite:MotionState .

m3-lite:RotationalSpeedEngine
        a                owl:Class ;
        rdfs:comment     "Rotational speed is a property that is the rate of rotation of a material around an axis, in this case the engine cylinders." ;
        rdfs:label       "Rotational Speed Engine"@en ;
        rdfs:seeAlso     "http://purl.oclc.org/NET/ssnx/qu/quantity#rotationalSpeed" ;
        rdfs:subClassOf  m3-lite:RotationalSpeed .

qudt_unit:ElectricCurrent
        a                owl:Class ;
        rdfs:comment     "Electric current is the flow of electric charge. It is a base quantity in the International System of Units. Electric current is electric charge divided by time. Electric Current is the flow (movement) of electric charge. The amount of electric current through some surface, e.g., a section through a copper conductor, is defined as the amount of electric charge flowing through that surface over time."@en ;
        rdfs:label       "Electric Current"@en ;
        rdfs:seeAlso     "http://qudt.org/vocab/quantity#ElectricCurrent" ;
        rdfs:subClassOf  qu:QuantityKind .

foaf:name  a    owl:AnnotationProperty .

m3-lite:Irrigation  a    owl:Class ;
        rdfs:comment     "An actuator to automatically irrigate or not."@en ;
        rdfs:label       "Irrigation"@en ;
        rdfs:subClassOf  iot-lite:ActuatingDevice ;
        rdfs:subClassOf  [ a                   owl:Restriction ;
                           owl:onProperty      m3-lite:domainOfInterest ;
                           owl:someValuesFrom  m3-lite:Agriculture
                         ] .

m3-lite:HouseholdApplianceTemperature
        a                owl:Class ;
        rdfs:comment     ""@en ;
        rdfs:label       "Household Appliance Temperature"@en ;
        rdfs:subClassOf  m3-lite:Temperature .

m3-lite:SaltMeter  a     owl:Class ;
        rdfs:comment     "Salt meter, salinity can be used in the fishery domain [Xiang Su et al. 2014]"@en ;
        rdfs:label       "Salt Meter"@en ;
        rdfs:subClassOf  ssn:SensingDevice ;
        rdfs:subClassOf  [ a                   owl:Restriction ;
                           owl:onProperty      m3-lite:domainOfInterest ;
                           owl:someValuesFrom  m3-lite:Environment
                         ] .

m3-lite:Wind  a          owl:Class ;
        rdfs:comment     "Wind"@en ;
        rdfs:label       "Wind"@en ;
        rdfs:subClassOf  m3-lite:Environment .

m3-lite:ChemicalAgentAtmosphericConcentrationAirParticles
        a                owl:Class ;
        rdfs:comment     "The concentration of air particles suspended in an atmosphere." ;
        rdfs:label       "Chemical Agent Atmospheric Concentration Air Particles" ;
        rdfs:subClassOf  m3-lite:ChemicalAgentAtmosphericConcentration .

m3-lite:Weight  a        owl:Class ;
        rdfs:comment     "Weight"@en ;
        rdfs:label       "Weight"@en ;
        rdfs:subClassOf  qu:QuantityKind .

m3-lite:BloodGlucose  a  owl:Class ;
        rdfs:comment     "Blood Glucose level, blood sugar level"@en ;
        rdfs:label       "Blood Glucose"@en ;
        rdfs:subClassOf  qu:QuantityKind .

m3-lite:Sink  a          owl:Class ;
        rdfs:comment     "An actuator to automatically switch on/off the sink."@en ;
        rdfs:label       "Sink"@en ;
        rdfs:subClassOf  iot-lite:ActuatingDevice ;
        rdfs:subClassOf  [ a                   owl:Restriction ;
                           owl:onProperty      m3-lite:domainOfInterest ;
                           owl:someValuesFrom  m3-lite:BuildingAutomation
                         ] .

qudt_unit:DegreeAngle
        a                owl:Class ;
        rdfs:comment     "A plane angle unit which is equal to 1/360 of a full rotation or pi/180 rad."@en ;
        rdfs:label       "Degree angle"@en ;
        rdfs:seeAlso     "http://qudt.org/vocab/unit#DegreeAngle" ;
        rdfs:subClassOf  m3-lite:Degree .

qu:Unit  a      owl:Class .

m3-lite:Wout  a          owl:Class ;
        rdfs:comment     "This unit is used to measure delta dew point within the Com4Innov tesbed. Natural number (W/out unit)"@en ;
        rdfs:label       "W/out"@en ;
        rdfs:subClassOf  qu:Unit .

m3-lite:WeatherLuminosity
        a                owl:Class ;
        rdfs:comment     ""@en ;
        rdfs:label       "Weather Luminosity"@en ;
        rdfs:subClassOf  m3-lite:Illuminance .

m3-lite:AirThermometer
        a                owl:Class ;
        rdfs:comment     "Air Thermometer"@en ;
        rdfs:label       "Air Thermometer"@en ;
        rdfs:subClassOf  ssn:SensingDevice ;
        rdfs:subClassOf  [ a                   owl:Restriction ;
                           owl:onProperty      m3-lite:domainOfInterest ;
                           owl:someValuesFrom  m3-lite:Agriculture
                         ] ;
        txn:hasImage     <http://sensormeasurement.appspot.com/images/sensor/thermometer.png> .

m3-lite:FrequencySensor
        a                owl:Class ;
        rdfs:comment     "Frequency Sensor"@en ;
        rdfs:label       "Frequency Sensor"@en ;
        rdfs:subClassOf  ssn:SensingDevice .

m3-lite:Direction  a     owl:Class ;
        rdfs:label       "Direction"@en ;
        rdfs:subClassOf  qu:QuantityKind .

m3-lite:AirQuality  a    owl:Class ;
        rdfs:comment     "An air quality index (AQI) is a number used by government agencies to communicate to the public how polluted the air currently is or how polluted it is forecast to become. Different countries have their own air quality indices, corresponding to different national air quality standards." ;
        rdfs:label       "Air Quality" ;
        rdfs:subClassOf  qu:QuantityKind .

m3-lite:Agriculture  a   owl:Class ;
        rdfs:comment     "Agriculture, Smart farm as an Internet of Things (IoT) applicative domain."@en ;
        rdfs:label       "Agriculture"@en ;
        rdfs:subClassOf  m3-lite:DomainOfInterest .

m3-lite:Angular  a       owl:Class ;
        rdfs:comment     "Angular"@en ;
        rdfs:label       "Angular"@en ;
        rdfs:subClassOf  qu:QuantityKind .

m3-lite:Temperature  a   owl:Class ;
        rdfs:comment     "By defaut, Air temperature"@en ;
        rdfs:label       "Temperature"@en ;
        rdfs:seeAlso     aws:air_temperature , openIoT:Temperature , <http://archive.knoesis.org/research/semsci/application_domain/sem_sensor/ont/sensor-observation.owlTemperatureProperty> ;
        rdfs:subClassOf  qu:QuantityKind .

m3-lite:Okta  a          owl:Class ;
        rdfs:comment     "Okta is the unit to measure the cloud cover"@en ;
        rdfs:label       "Okta"@en ;
        rdfs:subClassOf  qu:Unit .

m3-lite:NH3_Sensor  a    owl:Class ;
        rdfs:comment     ""@en ;
        rdfs:label       "NH3_Sensor"@en ;
        rdfs:subClassOf  m3-lite:GaseousPollutantSensor .

m3-lite:ElectricalSensor
        a                owl:Class ;
        rdfs:comment     "Electrical Sensor"@en ;
        rdfs:label       "Electrical Sensor"@en ;
        rdfs:subClassOf  ssn:SensingDevice .

m3-lite:KilometerPerHour
        a                owl:Class ;
        rdfs:label       "Kilometer Per Hour" ;
        rdfs:seeAlso     "http://data.qudt.org/qudt/owl/1.0.0/unit.owl#KilometerPerHour" ;
        rdfs:subClassOf  m3-lite:MeterPerSecond .

m3-lite:SkinConductanceSensor
        a                owl:Class ;
        rdfs:comment     "Skin Conductance Sensor"@en ;
        rdfs:label       "Skin Conductance Sensor"@en ;
        rdfs:subClassOf  ssn:SensingDevice ;
        rdfs:subClassOf  [ a                   owl:Restriction ;
                           owl:onProperty      m3-lite:domainOfInterest ;
                           owl:someValuesFrom  m3-lite:Health
                         ] ;
        rdfs:subClassOf  [ a                   owl:Restriction ;
                           owl:onProperty      m3-lite:domainOfInterest ;
                           owl:someValuesFrom  m3-lite:Emotion
                         ] .

m3-lite:Passport  a      owl:Class ;
        rdfs:comment     "An RFID tag is embedded on passport."@en ;
        rdfs:label       "Passport"@en ;
        rdfs:subClassOf  m3-lite:RFIDQuantityKind .

m3-lite:Transportation
        a                owl:Class ;
        rdfs:comment     "Transportation, Smart Car/Vehicle, Intelligent Transport System (ITS) as an Internet of Things (IoT) applicative domain"@en ;
        rdfs:label       "Transportation"@en ;
        rdfs:subClassOf  m3-lite:DomainOfInterest .

m3-lite:Time  a          owl:Class ;
        rdfs:comment     ""@en ;
        rdfs:label       "Time"@en ;
        rdfs:subClassOf  qu:Unit .

m3-lite:SystolicBloodPressure
        a                owl:Class ;
        rdfs:comment     ""@en ;
        rdfs:label       "Systolic Blood pressure"@en ;
        rdfs:subClassOf  m3-lite:BloodPressure .

m3-lite:Pollution  a     owl:Class ;
        rdfs:comment     ""@en ;
        rdfs:label       "Pollution"@en ;
        rdfs:subClassOf  m3-lite:Environment .

m3-lite:Odometer  a      owl:Class ;
        rdfs:comment     "An odometer or odograph is an instrument that indicates distance traveled by a vehicle, such as bicycle or automobile."@en ;
        rdfs:label       "Odometer"@en ;
        rdfs:subClassOf  ssn:SensingDevice .

m3-lite:NFC  a           owl:Class ;
        rdfs:comment     "A tagging device can be NFC (Near Field Communication)"@en ;
        rdfs:label       "NFC"@en ;
        rdfs:subClassOf  iot-lite:TagDevice .

dcterms:issued  a  owl:AnnotationProperty .

m3-lite:AirPollution  a  owl:Class ;
        rdfs:comment     "Air Pollution, Air Quality"@en ;
        rdfs:label       "Air Pollution"@en ;
        rdfs:subClassOf  qu:QuantityKind .

m3-lite:Milliampere  a   owl:Class ;
        rdfs:label       "Milliampere (mA)" ;
        rdfs:subClassOf  m3-lite:Ampere .

m3-lite:TrafficIntensity
        a                owl:Class ;
        rdfs:comment     "The intensity of a traffic flow is the number of vehicles passing a cross section of a road in a unit of time" ;
        rdfs:label       "Traffic Intensity"@en ;
        rdfs:subClassOf  qu:QuantityKind .

m3-lite:SoilHumiditySensor
        a                owl:Class ;
        rdfs:comment     "Soil Humidity sensor, Soil moisture, Hygrometer are an instrument used for measuring the soil moisture."@en ;
        rdfs:label       "Soil Humidity Sensor"@en ;
        rdfs:subClassOf  ssn:SensingDevice ;
        rdfs:subClassOf  [ a                   owl:Restriction ;
                           owl:onProperty      m3-lite:domainOfInterest ;
                           owl:someValuesFrom  m3-lite:Agriculture
                         ] .

m3-lite:GasDetector  a   owl:Class ;
        rdfs:comment     "Gas Detector"@en ;
        rdfs:label       "Gas Detector"@en ;
        rdfs:subClassOf  ssn:SensingDevice .

m3-lite:HeartBeatSensor
        a                owl:Class ;
        rdfs:comment     "HeartBeat Sensor, Heart rate, breath rate"@en ;
        rdfs:label       "Heart Beat Sensor"@en ;
        rdfs:subClassOf  ssn:SensingDevice ;
        rdfs:subClassOf  [ a                   owl:Restriction ;
                           owl:onProperty      m3-lite:domainOfInterest ;
                           owl:someValuesFrom  m3-lite:Health
                         ] ;
        txn:hasImage     <http://sensormeasurement.appspot.com/images/sensor/heartbeat.png> .

m3-lite:SpeedInstantaneous
        a                owl:Class ;
        rdfs:comment     "A measure of the instantaneous rate of motion of an object." ;
        rdfs:label       "Speed Instantaneous"@en ;
        rdfs:subClassOf  m3-lite:Speed .

m3-lite:Heating  a       owl:Class ;
        rdfs:comment     "An actuator to automatically switch on/off the heating."@en ;
        rdfs:label       "Heating"@en ;
        rdfs:subClassOf  iot-lite:ActuatingDevice ;
        rdfs:subClassOf  [ a                   owl:Restriction ;
                           owl:onProperty      m3-lite:domainOfInterest ;
                           owl:someValuesFrom  m3-lite:BuildingAutomation
                         ] .

m3-lite:Meter  a         owl:Class ;
        rdfs:comment     ""@en ;
        rdfs:label       "Meter"@en ;
        rdfs:seeAlso     sweet_unit:meter , qudt_unit:Meter ;
        rdfs:subClassOf  qu:Unit .

m3-lite:Millibar  a      owl:Class ;
        rdfs:label       "Millibar" ;
        rdfs:subClassOf  qudt_unit:Bar .

m3-lite:Mileage  a       owl:Class ;
        rdfs:label       "Mileage"@en ;
        rdfs:subClassOf  qu:QuantityKind .

m3-lite:Computer  a      owl:Class ;
        rdfs:comment     ""@en ;
        rdfs:label       "Computer, PC"@en ;
        rdfs:subClassOf  iot-lite:ActuatingDevice ;
        rdfs:subClassOf  [ a                   owl:Restriction ;
                           owl:onProperty      m3-lite:domainOfInterest ;
                           owl:someValuesFrom  m3-lite:BuildingAutomation
                         ] .

m3-lite:Longitude  a     owl:Class ;
        rdfs:comment     ""@en ;
        rdfs:label       "Longitude"@en ;
        rdfs:seeAlso     wgs84_pos:longitude ;
        rdfs:subClassOf  qu:Unit .

m3-lite:DishWasher  a    owl:Class ;
        rdfs:comment     "An actuator to automatically switch on/off the dishwasher."@en ;
        rdfs:label       "Dish Washer"@en ;
        rdfs:subClassOf  iot-lite:ActuatingDevice ;
        rdfs:subClassOf  [ a                   owl:Restriction ;
                           owl:onProperty      m3-lite:domainOfInterest ;
                           owl:someValuesFrom  m3-lite:BuildingAutomation
                         ] .

m3-lite:Thermometer  a   owl:Class ;
        rdfs:comment     "A thermometer to measure the temperature in a room or outside"@en ;
        rdfs:label       "Thermometer"@en ;
        rdfs:seeAlso     cose:TempuratureSensor , aws:TemperatureSensor ;
        rdfs:subClassOf  ssn:SensingDevice ;
        rdfs:subClassOf  [ a                   owl:Restriction ;
                           owl:onProperty      m3-lite:domainOfInterest ;
                           owl:someValuesFrom  m3-lite:Weather
                         ] ;
        rdfs:subClassOf  [ a                   owl:Restriction ;
                           owl:onProperty      m3-lite:domainOfInterest ;
                           owl:someValuesFrom  m3-lite:BuildingAutomation
                         ] ;
        rdfs:subClassOf  [ a                   owl:Restriction ;
                           owl:onProperty      m3-lite:domainOfInterest ;
                           owl:someValuesFrom  m3-lite:EnergyFOI
                         ] ;
        rdfs:subClassOf  [ a                   owl:Restriction ;
                           owl:onProperty      m3-lite:domainOfInterest ;
                           owl:someValuesFrom  m3-lite:Environment
                         ] ;
        txn:hasImage     <http://sensormeasurement.appspot.com/images/sensor/thermometer.png> .

m3-lite:WorkingState  a  owl:Class ;
        rdfs:label       "Working State"@en ;
        rdfs:subClassOf  qu:QuantityKind .

m3-lite:Day  a           owl:Class ;
        rdfs:comment     ""@en ;
        rdfs:label       "Day"@en ;
        rdfs:subClassOf  qu:Unit .

m3-lite:Energy  a        owl:Class ;
        rdfs:comment     "Measure procuded by energy meter"@en ;
        rdfs:label       "Energy"@en ;
        rdfs:subClassOf  qu:QuantityKind .

m3-lite:WaterTemperature
        a                owl:Class ;
        rdfs:comment     ""@en ;
        rdfs:label       "Water Temperature"@en ;
        rdfs:subClassOf  m3-lite:Temperature .

m3-lite:H2S_Sensor  a    owl:Class ;
        rdfs:comment     ""@en ;
        rdfs:label       "H2S_Sensor"@en ;
        rdfs:subClassOf  m3-lite:GaseousPollutantSensor .

m3-lite:Capacitance  a   owl:Class ;
        rdfs:comment     "Capacitance is the ability of a body to store an electric charge."@en ;
        rdfs:label       "Capacitance"@en ;
        rdfs:subClassOf  qu:QuantityKind .

m3-lite:DVD  a           owl:Class ;
        rdfs:comment     "An RFID tag is embedded on DVD."@en ;
        rdfs:label       "DVD"@en ;
        rdfs:seeAlso     movie:Movie ;
        rdfs:subClassOf  m3-lite:RFIDQuantityKind .

m3-lite:DeltaDewPointSensor
        a                owl:Class ;
        rdfs:comment     "Difference between Dewpoint and surface temperatures. The Com4Innov testbed is providing delta dew point sensor."@en ;
        rdfs:label       "Delta Dew Point Sensor"@en ;
        rdfs:subClassOf  ssn:SensingDevice .

m3-lite:TrafficJam  a    owl:Class ;
        rdfs:comment     ""@en ;
        rdfs:label       "TrafficJam"@en ;
        rdfs:subClassOf  m3-lite:Transportation .

m3-lite:SoilTemperature
        a                owl:Class ;
        rdfs:comment     "Soil temperature is the bulk temperature of the soil, not the surface (skin) temperature."@en ;
        rdfs:label       "Soil Temperature"@en ;
        rdfs:subClassOf  m3-lite:Temperature .

m3-lite:Toll  a          owl:Class ;
        rdfs:comment     "An RFID tag is embedded on electronic toll system."@en ;
        rdfs:label       "Toll"@en ;
        rdfs:subClassOf  m3-lite:RFIDQuantityKind .

m3-lite:SoundSensor  a   owl:Class ;
        rdfs:comment     "Sound Sensor, Noise level Sensor, Volume sensor, Microphone"@en ;
        rdfs:label       "Sound Sensor"@en ;
        rdfs:seeAlso     cose:Microphone ;
        rdfs:subClassOf  ssn:SensingDevice ;
        rdfs:subClassOf  [ a                   owl:Restriction ;
                           owl:onProperty      m3-lite:domainOfInterest ;
                           owl:someValuesFrom  m3-lite:Transportation
                         ] ;
        rdfs:subClassOf  [ a                   owl:Restriction ;
                           owl:onProperty      m3-lite:domainOfInterest ;
                           owl:someValuesFrom  m3-lite:BuildingAutomation
                         ] ;
        txn:hasImage     <http://sensormeasurement.appspot.com/images/sensor/noise.png> .

m3-lite:LuminousFlux  a  owl:Class ;
        rdfs:comment     "Luminous Flux is the measure of the perceived power of light."@en ;
        rdfs:label       "LuminousFlux"@en ;
        rdfs:subClassOf  qu:QuantityKind .

m3-lite:SolarRadiationSensor
        a                owl:Class ;
        rdfs:comment     "Solar Radiation Sensor. PAR (Photosynthetically Active Radiation) Sensor, Sun Light. Unit watts per square meter (w/m2)"@en ;
        rdfs:label       "Solar Radiation Sensor"@en ;
        rdfs:seeAlso     spitfire:Light , aws:RadiationSensor ;
        rdfs:subClassOf  ssn:SensingDevice ;
        rdfs:subClassOf  [ a                   owl:Restriction ;
                           owl:onProperty      m3-lite:domainOfInterest ;
                           owl:someValuesFrom  m3-lite:Agriculture
                         ] ;
        rdfs:subClassOf  [ a                   owl:Restriction ;
                           owl:onProperty      m3-lite:domainOfInterest ;
                           owl:someValuesFrom  m3-lite:Weather
                         ] ;
        txn:hasImage     <http://sensormeasurement.appspot.com/images/sensor/solarRadiation.png> .

m3-lite:Hour  a          owl:Class ;
        rdfs:comment     ""@en ;
        rdfs:label       "Hour"@en ;
        rdfs:seeAlso     sweet_unit:hour ;
        rdfs:subClassOf  qu:Unit .

m3-lite:ParkingSpace  a  owl:Class ;
        rdfs:comment     "An RFID tag is embedded on parking space to detect if they are available or not."@en ;
        rdfs:label       "ParkingSpace"@en ;
        rdfs:subClassOf  m3-lite:RFIDQuantityKind .

m3-lite:MicrogramPerCubicMetre
        a                owl:Class ;
        rdfs:comment     "Microgram per cubic metre is a unit of density defined as microgram divided by cubic metre. Milligram per cubic metre is a derived unit in the International System of Units." ;
        rdfs:label       "MicrogramPerCubicMetre, MicrogramPerCubicMeter" ;
        rdfs:seeAlso     "http://purl.oclc.org/NET/ssnx/qu/unit#microgramPerCubicMetre" ;
        rdfs:subClassOf  m3-lite:GramPerCubicMetre .

m3-lite:Sound  a         owl:Class ;
        rdfs:comment     ""@en ;
        rdfs:label       "Sound, noise level"@en ;
        rdfs:subClassOf  qu:QuantityKind .

m3-lite:SoilMoistureTension
        a                owl:Class ;
        rdfs:comment     "The force per unit area required to remove film water from soil." ;
        rdfs:label       "Soil Moisture Tension"@en ;
        rdfs:subClassOf  qu:QuantityKind .

m3-lite:Decibel_A  a     owl:Class ;
        rdfs:comment     "A ratio unit which is an indicator of sound power per unit area." ;
        rdfs:label       "Decibel (db)"@en ;
        rdfs:subClassOf  m3-lite:Decibel .

m3-lite:ShakeSensor  a   owl:Class ;
        rdfs:comment     "Shake sensors can deduce the quality of the road, earthquakes."@en ;
        rdfs:label       "Shake Sensor"@en ;
        rdfs:seeAlso     cose:ShakeSensor ;
        rdfs:subClassOf  ssn:SensingDevice ;
        rdfs:subClassOf  [ a                   owl:Restriction ;
                           owl:onProperty      m3-lite:domainOfInterest ;
                           owl:someValuesFrom  m3-lite:Environment
                         ] ;
        rdfs:subClassOf  [ a                   owl:Restriction ;
                           owl:onProperty      m3-lite:domainOfInterest ;
                           owl:someValuesFrom  m3-lite:Transportation
                         ] .

m3-lite:FuelConsumptionInstantaneous
        a                owl:Class ;
        rdfs:comment     "A measure that displays the instantaneous fuel consumption of a vehicle during its operation." ;
        rdfs:label       "Fuel Consumption Instantaneous"@en ;
        rdfs:subClassOf  m3-lite:FuelConsumption .

m3-lite:ConductivitySensor
        a                owl:Class ;
        rdfs:comment     "Salinity"@en ;
        rdfs:label       "Conductivity Sensor"@en ;
        rdfs:subClassOf  ssn:SensingDevice .

m3-lite:Tonne  a         owl:Class ;
        rdfs:comment     ""@en ;
        rdfs:label       "Tonne"@en ;
        rdfs:subClassOf  qu:Unit .

m3-lite:GyrometerSensor
        a                owl:Class ;
        rdfs:comment     "A gyrometer is an instrument which measures an angular speed."@en ;
        rdfs:label       "Gyrometer Sensor"@en ;
        rdfs:subClassOf  ssn:SensingDevice ;
        rdfs:subClassOf  [ a                   owl:Restriction ;
                           owl:onProperty      m3-lite:domainOfInterest ;
                           owl:someValuesFrom  m3-lite:Transportation
                         ] .

m3-lite:Var  a           owl:Class ;
        rdfs:comment     "In electric power transmission and distribution, volt-ampere reactive (var) is a unit in which reactive power is expressed in an AC electric power system." ;
        rdfs:label       "Var"@en ;
        rdfs:seeAlso     "http://purl.oclc.org/NET/ssnx/qu/unit#var" ;
        rdfs:subClassOf  qu:Unit .

m3-lite:ChemicalAgentAtmosphericConcentrationNO2
        a                owl:Class ;
        rdfs:comment     "The concentration of NO2 gas suspended in an atmosphere." ;
        rdfs:label       "Chemical Agent Atmospheric Concentration NO2" ;
        rdfs:subClassOf  m3-lite:ChemicalAgentAtmosphericConcentration .

m3-lite:TV  a            owl:Class ;
        rdfs:comment     "An actuator to automatically switch on/off the television."@en ;
        rdfs:label       "TV"@en ;
        rdfs:subClassOf  iot-lite:ActuatingDevice ;
        rdfs:subClassOf  [ a                   owl:Restriction ;
                           owl:onProperty      m3-lite:domainOfInterest ;
                           owl:someValuesFrom  m3-lite:BuildingAutomation
                         ] .

m3-lite:Clothing  a      owl:Class ;
        rdfs:comment     "An RFID tag is embedded on clothes."@en ;
        rdfs:label       "Clothes"@en ;
        rdfs:subClassOf  m3-lite:RFIDQuantityKind .

m3-lite:Cholesterol  a   owl:Class ;
        rdfs:comment     "Cholesterol measurement"@en ;
        rdfs:label       "Cholesterol"@en ;
        rdfs:subClassOf  qu:QuantityKind .

m3-lite:BuildingAutomation
        a                owl:Class ;
        rdfs:comment     "Smart Home/Building Automation as an Internet of Things (IoT) applicative domain."@en ;
        rdfs:label       "Smart Building"@en ;
        rdfs:seeAlso     dogont:BuildingEnvironment ;
        rdfs:subClassOf  m3-lite:DomainOfInterest .

m3-lite:PulseOxymeter
        a                owl:Class ;
        rdfs:comment     "Pulse Oxymeter, SpO2, Blood Oxygen Saturation Sensor are used to measure the concentration of oxygen in the blood."@en ;
        rdfs:label       "Pulse Oxymeter"@en ;
        rdfs:subClassOf  ssn:SensingDevice ;
        rdfs:subClassOf  [ a                   owl:Restriction ;
                           owl:onProperty      m3-lite:domainOfInterest ;
                           owl:someValuesFrom  m3-lite:Health
                         ] .

m3-lite:Latitude  a      owl:Class ;
        rdfs:comment     ""@en ;
        rdfs:label       "Latitude"@en ;
        rdfs:seeAlso     wgs84_pos:latitude ;
        rdfs:subClassOf  qu:Unit .

m3-lite:CO_Sensor  a     owl:Class ;
        rdfs:comment     "Carbon Monoxide (CO) Sensor"@en ;
        rdfs:label       "Carbon Monoxide (CO) Sensor"@en ;
        rdfs:subClassOf  m3-lite:GaseousPollutantSensor .

m3-lite:TimeRelatedState
        a                owl:Class ;
        rdfs:label       "Time Related State"@en ;
        rdfs:subClassOf  qu:QuantityKind .

m3-lite:BeatPerMinute
        a                owl:Class ;
        rdfs:comment     "BeatPerMinute (bpm) is the unit to measure heart rate"@en ;
        rdfs:label       "Beat Per Minute (bpm)"@en ;
        rdfs:subClassOf  qu:Unit .

m3-lite:BoardTemperature
        a                owl:Class ;
        rdfs:label       "Board Temperature"@en ;
        rdfs:subClassOf  m3-lite:Temperature .

m3-lite:Methane_Sensor
        a                owl:Class ;
        rdfs:comment     "Methane (CH4) Sensor"@en ;
        rdfs:label       "Methane (CH4) Sensor"@en ;
        rdfs:subClassOf  m3-lite:GaseousPollutantSensor .

m3-lite:SunPositionDirection
        a                owl:Class ;
        rdfs:comment     "To detect sun from north eastm, south or west. Unit Degree"@en ;
        rdfs:label       "Sun Position Direction"@en ;
        rdfs:subClassOf  qu:QuantityKind .

m3-lite:City  a          owl:Class ;
        rdfs:comment     "Smart City as an Internet of Things (IoT) applicative domain."@en ;
        rdfs:label       "Smart City"@en ;
        rdfs:subClassOf  m3-lite:DomainOfInterest .

m3-lite:ChemicalAgentAtmosphericConcentrationCO
        a                owl:Class ;
        rdfs:comment     "The concentration of CO gas suspended in an atmosphere." ;
        rdfs:label       "Chemical Agent Atmospheric Concentration CO" ;
        rdfs:subClassOf  m3-lite:ChemicalAgentAtmosphericConcentration .

m3-lite:Gauss  a         owl:Class ;
        rdfs:comment     "Gauss is a unit."@en ;
        rdfs:label       "Gauss"@en ;
        rdfs:subClassOf  qu:Unit .

m3-lite:Second_angle  a  owl:Class ;
        rdfs:comment     ""@en ;
        rdfs:label       "Second angle"@en ;
        rdfs:subClassOf  qu:Unit .

m3-lite:ElectricField2400MHz
        a                owl:Class ;
        rdfs:comment     "A field of force associated with a moving electric charge equivalent to an electric field and a magnetic field at right angles to each other and to the direction of propagation. Applied to the 2400 MHz UHF band." ;
        rdfs:label       "Electric Field 2400 MHz"@en ;
        rdfs:subClassOf  m3-lite:ElectricField .

m3-lite:SO2_Sensor  a    owl:Class ;
        rdfs:comment     "Sulfur Dioxide (SO2) Sensor"@en ;
        rdfs:label       "Sulfur Dioxide (SO2) Sensor"@en ;
        rdfs:subClassOf  m3-lite:GaseousPollutantSensor .

m3-lite:Volt  a          owl:Class ;
        rdfs:comment     ""@en ;
        rdfs:label       "Volt"@en ;
        rdfs:seeAlso     sweet_unit:volt ;
        rdfs:subClassOf  qu:Unit .

m3-lite:Millilitre  a    owl:Class ;
        rdfs:comment     "Millilitre, Milliliter" ;
        rdfs:label       "Millilitre" ;
        rdfs:subClassOf  m3-lite:Liter .

m3-lite:PositionAltitude
        a                owl:Class ;
        rdfs:comment     "The vertical distance above mean sea level." ;
        rdfs:label       "Position Altitude"@en ;
        rdfs:seeAlso     "http://sweet.jpl.nasa.gov/2.3/propSpaceHeight.owl#Altitude" ;
        rdfs:subClassOf  m3-lite:Position .

m3-lite:FallDetector  a  owl:Class ;
        rdfs:comment     "Fall detectors to detect if elderly people falls."@en ;
        rdfs:label       "Fall Detector"@en ;
        rdfs:subClassOf  ssn:SensingDevice ;
        rdfs:subClassOf  [ a                   owl:Restriction ;
                           owl:onProperty      m3-lite:domainOfInterest ;
                           owl:someValuesFrom  m3-lite:BuildingAutomation
                         ] ;
        txn:hasImage     <http://sensormeasurement.appspot.com/images/sensor/fall.png> .

m3-lite:chemicalAgentAtmosphericConcentrationO3
        a                owl:Class ;
        rdfs:comment     "The concentration of ozone (O3) gas suspended in an atmosphere." ;
        rdfs:label       "Chemical Agent Atmospheric Concentration O3"@en ;
        rdfs:subClassOf  m3-lite:ChemicalAgentAtmosphericConcentration .

m3-lite:ElectricField1800MHz
        a                owl:Class ;
        rdfs:comment     "A field of force associated with a moving electric charge equivalent to an electric field and a magnetic field at right angles to each other and to the direction of propagation. Applied to the 1800 MHz UHF band." ;
        rdfs:label       "Electric Field 1800 MHz"@en ;
        rdfs:subClassOf  m3-lite:ElectricField .

m3-lite:NO2_Sensor  a    owl:Class ;
        rdfs:comment     "E.g. provided by OpenIoT, gas sensor detecting levels of nitrogen dioxide (NO2)"@en ;
        rdfs:label       "Nitrogen Dioxide (NO2) Sensor"@en ;
        rdfs:subClassOf  m3-lite:GaseousPollutantSensor ;
        rdfs:subClassOf  [ a                   owl:Restriction ;
                           owl:onProperty      m3-lite:domainOfInterest ;
                           owl:someValuesFrom  m3-lite:Environment
                         ] .

m3-lite:AtmosphericPressure
        a                owl:Class ;
        rdfs:comment     "The pressure exerted by the atmosphere as a consequence of gravitational attraction exerted upon the column of air lying directly above the point in question."@en ;
        rdfs:label       "Atmospheric Pressure"@en ;
        rdfs:seeAlso     "http://purl.oclc.org/NET/ssnx/qu/quantity#atmosphericPressure" ;
        rdfs:seeAlso     shw:AtmosphericPressure , openIoT:AtmospherePressure ;
        rdfs:subClassOf  m3-lite:Pressure .

m3-lite:TrackingCD  a    owl:Class ;
        rdfs:comment     ""@en ;
        rdfs:label       "Tracking CD"@en ;
        rdfs:subClassOf  m3-lite:TrackingGood .

m3-lite:O3_Sensor  a     owl:Class ;
        rdfs:comment     "E.g. provided by OpenIoT, gas sensor detecting levels of ozone (O3)"@en ;
        rdfs:label       "Ozone (O3) Level Sensor"@en ;
        rdfs:subClassOf  m3-lite:GaseousPollutantSensor .

m3-lite:FuelConsumptionTotal
        a                owl:Class ;
        rdfs:comment     "Accumulated amount of fuel used during vehicle operation." ;
        rdfs:label       "Fuel Consumption Total"@en ;
        rdfs:subClassOf  m3-lite:FuelConsumption .

m3-lite:DirectionAzimuth
        a                owl:Class ;
        rdfs:comment     "The geodetic azimuth of the direction towards which an object is moving." ;
        rdfs:label       "Direction Azimuth"@en ;
        rdfs:subClassOf  m3-lite:Direction .

qu:QuantityKind  a  owl:Class .

m3-lite:RotationalSpeed
        a                owl:Class ;
        rdfs:label       "Rotational Speed"@en ;
        rdfs:subClassOf  qu:QuantityKind .

m3-lite:ElectricField
        a                owl:Class ;
        rdfs:label       "Electric Field"@en ;
        rdfs:seeAlso     "http://qudt.org/vocab/quantity#ElectricField" ;
        rdfs:subClassOf  qu:QuantityKind .

m3-lite:Conductivity  a  owl:Class ;
        rdfs:comment     ""@en ;
        rdfs:label       "Conductivity"@en ;
        rdfs:subClassOf  qu:QuantityKind .

m3-lite:TemperatureEngine
        a                owl:Class ;
        rdfs:comment     "The temperature of a vehicle engine." ;
        rdfs:label       "Temperature Engine" ;
        rdfs:subClassOf  m3-lite:Temperature .

m3-lite:SunPositionElevation
        a                owl:Class ;
        rdfs:comment     "To detect sun state (day, twilight, night, etc). Unit Degree"@en ;
        rdfs:label       "Sun Position Elevation"@en ;
        rdfs:subClassOf  qu:QuantityKind .

m3-lite:BoardThermometer
        a                owl:Class ;
        rdfs:comment     "Board Thermometer is provided by the Com4Innov testbed."@en ;
        rdfs:label       "Board Thermometer"@en ;
        rdfs:subClassOf  ssn:SensingDevice ;
        txn:hasImage     <http://sensormeasurement.appspot.com/images/sensor/thermometer.png> .

m3-lite:Year  a          owl:Class ;
        rdfs:comment     "Year"@en ;
        rdfs:label       "Year"@en ;
        rdfs:seeAlso     sweet_unit:year ;
        rdfs:subClassOf  qu:Unit .

m3-lite:ElectricCharge
        a                owl:Class ;
        rdfs:comment     ""@en ;
        rdfs:label       "Electric Charge"@en ;
        rdfs:subClassOf  qu:QuantityKind .

m3-lite:TrackingPassport
        a                owl:Class ;
        rdfs:comment     ""@en ;
        rdfs:label       "Tracking Passport"@en ;
        rdfs:subClassOf  m3-lite:TrackingGood .

m3-lite:Mass  a          owl:Class ;
        rdfs:comment     "Mass is a property that is a constant that indicates the resistance of a material against acceleration." ;
        rdfs:label       "Mass"@en ;
        rdfs:seeAlso     "http://purl.oclc.org/NET/ssnx/qu/quantity#mass" ;
        rdfs:subClassOf  qu:QuantityKind .

m3-lite:HumiditySensor
        a                owl:Class ;
        rdfs:comment     "Humidity sensor or hygrometer is an instrument used for measuring the moisture concent in the environment."@en ;
        rdfs:label       "Humidity Sensor"@en ;
        rdfs:seeAlso     aws:HumiditySensor ;
        rdfs:subClassOf  ssn:SensingDevice ;
        rdfs:subClassOf  [ a                   owl:Restriction ;
                           owl:onProperty      m3-lite:domainOfInterest ;
                           owl:someValuesFrom  m3-lite:Weather
                         ] ;
        rdfs:subClassOf  [ a                   owl:Restriction ;
                           owl:onProperty      m3-lite:domainOfInterest ;
                           owl:someValuesFrom  m3-lite:Agriculture
                         ] ;
        rdfs:subClassOf  [ a                   owl:Restriction ;
                           owl:onProperty      m3-lite:domainOfInterest ;
                           owl:someValuesFrom  m3-lite:Environment
                         ] .

m3-lite:PositionLatitude
        a                owl:Class ;
        rdfs:comment     "The angular distance north or south from the equator of a point on the earth's surface, measured on the meridian of the point." ;
        rdfs:label       "Position Latitude"@en ;
        rdfs:seeAlso     "http://sweet.jpl.nasa.gov/2.3/reprSpaceCoordinate.owl#Latitude" ;
        rdfs:subClassOf  m3-lite:Position .

m3-lite:Humidity  a      owl:Class ;
        rdfs:comment     ""@en ;
        rdfs:label       "Humidity"@en ;
        rdfs:seeAlso     shw:Humidity , openIoT:AtmosphereHumidity , dogont:HumidityMeasurementMNotification ;
        rdfs:subClassOf  qu:QuantityKind .

m3-lite:PresenceState
        a                owl:Class ;
        rdfs:label       "Presence State"@en ;
        rdfs:seeAlso     "http://elite.polito.it/ontologies/dogont.owl#PresenceState" ;
        rdfs:subClassOf  qu:QuantityKind .

m3-lite:WashingMachine
        a                owl:Class ;
        rdfs:comment     "An actuator to automatically switch on/off the washing machine."@en ;
        rdfs:label       "Washing Machine"@en ;
        rdfs:subClassOf  iot-lite:ActuatingDevice ;
        rdfs:subClassOf  [ a                   owl:Restriction ;
                           owl:onProperty      m3-lite:domainOfInterest ;
                           owl:someValuesFrom  m3-lite:BuildingAutomation
                         ] .

m3-lite:FogLamp  a       owl:Class ;
        rdfs:comment     "The actuator fog lamp (on/off)"@en ;
        rdfs:label       "Fog lamp Actuator"@en ;
        rdfs:subClassOf  iot-lite:ActuatingDevice ;
        rdfs:subClassOf  [ a                   owl:Restriction ;
                           owl:onProperty      m3-lite:domainOfInterest ;
                           owl:someValuesFrom  m3-lite:Transportation
                         ] ;
        txn:hasImage     <http://sensormeasurement.appspot.com/images/sensor/fogLamp.png> .

m3-lite:SoundPressureLevel
        a                owl:Class ;
        rdfs:comment     "Sound pressure level is a logarithmic measure of the RMS sound pressure of a sound relative to a reference value, the threshold of hearing. The reference sound pressure was chosen conventionally to correspond to the quietest sound at 1000 Hz that the human ear can detect (20 uPa). In this case, the specific parameter is measured in an open environment." ;
        rdfs:label       "Sound Pressure Level"@en ;
        rdfs:seeAlso     "http://purl.oclc.org/NET/ssnx/qu/quantity#soundPressure" ;
        rdfs:subClassOf  qu:QuantityKind .

m3-lite:SolarRadiation
        a                owl:Class ;
        rdfs:comment     ""@en ;
        rdfs:label       "SolarRadiationMeasurement, PAR Measurement (Photosynthetically Active Radiation),"@en ;
        rdfs:subClassOf  qu:QuantityKind .

m3-lite:BloodPressure
        a                owl:Class ;
        rdfs:comment     ""@en ;
        rdfs:label       "Blood pressure"@en ;
        rdfs:subClassOf  m3-lite:Pressure .

m3-lite:PrecipitationSensor
        a                owl:Class ;
        rdfs:comment     "Precipitation Sensor, Pluviometer or Rainfall sensor is a sensor measuring the amount of precipitation/rainfall."@en ;
        rdfs:label       "Precipitation Sensor"@en ;
        rdfs:seeAlso     aws:PrecipitationSensor ;
        rdfs:subClassOf  ssn:SensingDevice ;
        rdfs:subClassOf  [ a                   owl:Restriction ;
                           owl:onProperty      m3-lite:domainOfInterest ;
                           owl:someValuesFrom  m3-lite:Weather
                         ] ;
        rdfs:subClassOf  [ a                   owl:Restriction ;
                           owl:onProperty      m3-lite:domainOfInterest ;
                           owl:someValuesFrom  m3-lite:Agriculture
                         ] ;
        txn:hasImage     <http://sensormeasurement.appspot.com/images/sensor/rain.png> .

m3-lite:DeltaDewPoint
        a                owl:Class ;
        rdfs:comment     "Difference between Dewpoint and surface temperatures" ;
        rdfs:label       "Delta Dew Point"@en ;
        rdfs:subClassOf  m3-lite:DewPoint .

m3-lite:MeterPerSecond
        a                owl:Class ;
        rdfs:comment     "A speed/velocity unit which is equal to the speed of an object traveling 1 meter distance in one second."@en ;
        rdfs:label       "Meter Per Second (m/s)"@en ;
        rdfs:seeAlso     "http://purl.oclc.org/NET/ssnx/qu/unit#metrePerSecond" ;
        rdfs:seeAlso     qudt_unit:MeterPerSecond ;
        rdfs:subClassOf  qu:Unit .

m3-lite:Emotion  a       owl:Class ;
        rdfs:comment     "Affective Science, Emotion, Mood, Emotional State, Brain Wave as an Internet of Things (IoT) applicative domain."@en ;
        rdfs:label       "Emotion"@en ;
        rdfs:seeAlso     naturopathy:Emotion , emoca:Emotion ;
        rdfs:subClassOf  m3-lite:DomainOfInterest .

m3-lite:Watt  a          owl:Class ;
        rdfs:comment     ""@en ;
        rdfs:label       "Watt (W)"@en ;
        rdfs:seeAlso     sweet_unit:watt ;
        rdfs:subClassOf  qu:Unit .

m3-lite:WindSpeed  a     owl:Class ;
        rdfs:comment     "The ratio of the distance covered by moving air to the time quantity taken to cover it."@en ;
        rdfs:label       "Wind Velocity/ Wind Speed"@en ;
        rdfs:seeAlso     openIoT:WindSpeed ;
        rdfs:subClassOf  qu:QuantityKind .

m3-lite:LuminousIntensity
        a                owl:Class ;
        rdfs:comment     ""@en ;
        rdfs:label       "Luminous Intensity"@en ;
        rdfs:subClassOf  qu:QuantityKind .

m3-lite:ElectricPotential
        a                owl:Class ;
        rdfs:comment     "Electric potential is the potential energy per unit charge associated with static (time-invariant) electric field."@en ;
        rdfs:label       "Electric Potential"@en ;
        rdfs:seeAlso     "http://purl.oclc.org/NET/ssnx/qu/dim#ElectricPotential" ;
        rdfs:subClassOf  qu:QuantityKind .

m3-lite:PositionLongitude
        a                owl:Class ;
        rdfs:comment     "The angular distance east or west on the earth's surface, measured by the angle contained between the meridian of a particular place and some prime meridian, as that of Greenwich, England, and expressed either in degrees or by some corresponding difference in time." ;
        rdfs:label       "Position Longitude"@en ;
        rdfs:seeAlso     "http://sweet.jpl.nasa.gov/2.3/reprSpaceCoordinate.owl#Longitude" ;
        rdfs:subClassOf  m3-lite:Position .

m3-lite:SmokeDetector
        a                owl:Class ;
        rdfs:comment     "Smoke detectors/Fire Alarms can detect if there is a fire, the smoke."@en ;
        rdfs:label       "Smoke Detector"@en ;
        rdfs:seeAlso     cose:SmokeAlarm ;
        rdfs:subClassOf  ssn:SensingDevice ;
        rdfs:subClassOf  [ a                   owl:Restriction ;
                           owl:onProperty      m3-lite:domainOfInterest ;
                           owl:someValuesFrom  m3-lite:BuildingAutomation
                         ] ;
        txn:hasImage     <http://sensormeasurement.appspot.com/images/sensor/smoke.png> .

m3-lite:domainOfInterest
        a             owl:ObjectProperty ;
        rdfs:comment  "This property is used to classify devices by DomainOfInterest (e.g., blood pressure sensor is used in healthcare)"@en ;
        rdfs:label    "domainOfInterest"@en ;
        rdfs:range    m3-lite:DomainOfInterest .

m3-lite:Radian  a        owl:Class ;
        rdfs:comment     ""@en ;
        rdfs:label       "Radian"@en ;
        rdfs:seeAlso     sweet_unit:radian ;
        rdfs:subClassOf  qu:Unit .

m3-lite:Soil  a          owl:Class ;
        rdfs:comment     "Environment"@en ;
        rdfs:label       "Environment"@en ;
        rdfs:subClassOf  m3-lite:Environment .

m3-lite:RFIDQuantityKind
        a                owl:Class ;
        rdfs:comment     ""@en ;
        rdfs:label       "RFID Measurement Type"@en ;
        rdfs:subClassOf  qu:QuantityKind .

m3-lite:BodyTemperature
        a                owl:Class ;
        rdfs:comment     ""@en ;
        rdfs:label       "Body Temperature"@en ;
        rdfs:subClassOf  m3-lite:Temperature .

m3-lite:CO2_Sensor  a    owl:Class ;
        rdfs:comment     "Carbon Dioxide (CO2) Sensor is used to measure air quality."@en ;
        rdfs:label       "Carbon Dioxide (CO2) Sensor"@en ;
        rdfs:subClassOf  m3-lite:GaseousPollutantSensor ;
        rdfs:subClassOf  [ a                   owl:Restriction ;
                           owl:onProperty      m3-lite:domainOfInterest ;
                           owl:someValuesFrom  m3-lite:Environment
                         ] ;
        rdfs:subClassOf  [ a                   owl:Restriction ;
                           owl:onProperty      m3-lite:domainOfInterest ;
                           owl:someValuesFrom  m3-lite:Agriculture
                         ] .

m3-lite:Illuminance  a   owl:Class ;
        rdfs:comment     "Illuminance is the total luminous flux incident on a surface, per unit area."@en ;
        rdfs:label       "Illuminance"@en ;
        rdfs:subClassOf  qu:QuantityKind .

m3-lite:Volt-ampere_reactive
        a                owl:Class ;
        rdfs:comment     "In electric power transmission and distribution, volt-ampere reactive (var) is a unit in which reactive power is expressed in an AC electric power system." ;
        rdfs:label       "Volt-ampere reactive, var" , "var" ;
        rdfs:seeAlso     "http://purl.oclc.org/NET/ssnx/qu/unit#var" ;
        rdfs:subClassOf  qu:Unit .

m3-lite:MagneticFluxDensity
        a                owl:Class ;
        rdfs:comment     ""@en ;
        rdfs:label       "MagneticFluxDensity"@en ;
        rdfs:subClassOf  qu:QuantityKind .

m3-lite:PressureSensor
        a                owl:Class ;
        rdfs:comment     "A pressure sensor can be attached on the bed to infer if the user is lying, sleeping, sitting, bed occupancy, etc."@en ;
        rdfs:label       "Pressure Sensor (e.g., bed)"@en ;
        rdfs:subClassOf  ssn:SensingDevice ;
        rdfs:subClassOf  [ a                   owl:Restriction ;
                           owl:onProperty      m3-lite:domainOfInterest ;
                           owl:someValuesFrom  m3-lite:BuildingAutomation
                         ] .

vann:preferredNamespaceUri
        a       owl:AnnotationProperty .

dc:description  a  owl:AnnotationProperty .

m3-lite:SunPositionElevationSensor
        a                owl:Class ;
        rdfs:comment     "To detect sun state (day, twilight, night, etc). Unit Degree"@en ;
        rdfs:label       "Sun Position Elevation Sensor"@en ;
        rdfs:subClassOf  ssn:SensingDevice ;
        rdfs:subClassOf  [ a                   owl:Restriction ;
                           owl:onProperty      m3-lite:domainOfInterest ;
                           owl:someValuesFrom  m3-lite:Weather
                         ] .

m3-lite:MilligramPerCubicMetre
        a                owl:Class ;
        rdfs:label       "MilligramPerCubicMetre, MilligramPerCubicMeter" ;
        rdfs:subClassOf  m3-lite:GramPerCubicMetre .

m3-lite:Rainfall  a      owl:Class ;
        rdfs:comment     "The depth of precipitation (water-equivalent) that accumulated over a measurement time quantity" ;
        rdfs:label       "Rainfall"@en ;
        rdfs:seeAlso     "http://sweet.jpl.nasa.gov/ontology/property.owl#Rainfall" ;
        rdfs:subClassOf  qu:QuantityKind .

ssn:SensingDevice  a     owl:Class ;
        rdfs:subClassOf  ssn:Device .

m3-lite:Centimetre  a    owl:Class ;
        rdfs:label       "Centimetre, Centimeter" ;
        rdfs:subClassOf  m3-lite:Meter .

m3-lite:MileageDistanceToService
        a                owl:Class ;
        rdfs:comment     "The distance which can be travelled by the vehicle before the next service inspection is required.  A negative distance is transmitted if the service inspection has been passed." ;
        rdfs:label       "Mileage Distance To Service"@en ;
        rdfs:subClassOf  m3-lite:Mileage .

m3-lite:Hotel  a         owl:Class ;
        rdfs:comment     ""@en ;
        rdfs:label       "Hotel"@en ;
        rdfs:subClassOf  m3-lite:Place .

m3-lite:Altitude  a      owl:Class ;
        rdfs:comment     "Altitude"@en ;
        rdfs:label       "Altitude"@en ;
        rdfs:subClassOf  qu:Unit .

m3-lite:BodyThermometer
        a                owl:Class ;
        rdfs:comment     "Body Thermometer"@en ;
        rdfs:label       "Body Thermometer"@en ;
        rdfs:subClassOf  ssn:SensingDevice ;
        rdfs:subClassOf  [ a                   owl:Restriction ;
                           owl:onProperty      m3-lite:domainOfInterest ;
                           owl:someValuesFrom  m3-lite:Health
                         ] ;
        txn:hasImage     <http://sensormeasurement.appspot.com/images/sensor/bodyThermometer.png> .

m3-lite:SkinConductance
        a                owl:Class ;
        rdfs:comment     "Skin conductance (or GSR: Galvanic Skin Response)"@en ;
        rdfs:label       "Skin conductance/ GSR"@en ;
        rdfs:subClassOf  qu:QuantityKind ;
        dc:description   "Electroderal activity (also known as skin conductance or galvanic skin response) directly correlates to the sympathetic nervous system activity and thus provides a powerful tool for monitoring arousal and certain aspects of autonomic regulation."@en .

dcterms:modified  a  owl:AnnotationProperty .

m3-lite:Health  a        owl:Class ;
        rdfs:comment     "Healthcare as an Internet of Things (IoT) applicative domain."@en ;
        rdfs:label       "Healthcare"@en ;
        rdfs:subClassOf  m3-lite:DomainOfInterest .

m3-lite:RFID  a          owl:Class ;
        rdfs:comment     "A tagging device can be RFID"@en ;
        rdfs:label       "RFID"@en ;
        rdfs:subClassOf  iot-lite:TagDevice .

m3-lite:NumberStep  a    owl:Class ;
        rdfs:comment     "NumberStep"@en ;
        rdfs:label       "NumberStep"@en ;
        rdfs:subClassOf  qu:QuantityKind .

m3-lite:Animal  a        owl:Class ;
        rdfs:comment     "An RFID tag is embedded on animal."@en ;
        rdfs:label       "Animal"@en ;
        rdfs:subClassOf  m3-lite:RFIDQuantityKind .

m3-lite:RoadTemperature
        a                owl:Class ;
        rdfs:comment     ""@en ;
        rdfs:label       "Road Temperature"@en ;
        rdfs:subClassOf  m3-lite:Temperature .

m3-lite:TransitPass  a   owl:Class ;
        rdfs:comment     "CommutationTicket/ Transit pass"@en ;
        rdfs:label       "TransitPass"@en ;
        rdfs:subClassOf  m3-lite:RFIDQuantityKind .

m3-lite:Distance  a      owl:Class ;
        rdfs:comment     ""@en ;
        rdfs:label       "Distance"@en ;
        rdfs:subClassOf  qu:QuantityKind .

m3-lite:WindChillSensor
        a                owl:Class ;
        rdfs:comment     "Wind Chill Sensor"@en ;
        rdfs:label       "Wind Chill Sensor"@en ;
        rdfs:subClassOf  ssn:SensingDevice ;
        rdfs:subClassOf  [ a                   owl:Restriction ;
                           owl:onProperty      m3-lite:domainOfInterest ;
                           owl:someValuesFrom  m3-lite:Weather
                         ] .

m3-lite:Freezer  a       owl:Class ;
        rdfs:comment     "An actuator to automatically open/close the freezer."@en ;
        rdfs:label       "Freezer, chiller"@en ;
        rdfs:subClassOf  iot-lite:ActuatingDevice ;
        rdfs:subClassOf  [ a                   owl:Restriction ;
                           owl:onProperty      m3-lite:domainOfInterest ;
                           owl:someValuesFrom  m3-lite:BuildingAutomation
                         ] .

m3-lite:TrackingTransitPass
        a                owl:Class ;
        rdfs:comment     ""@en ;
        rdfs:label       "Tracking TransitPass"@en ;
        rdfs:subClassOf  m3-lite:TrackingGood .

m3-lite:DewPointTemperature
        a                owl:Class ;
        rdfs:comment     "The temperature at which dew forms and is a measure of atmospheric moisture. It is the temperature to which air must be cooled at constant pressure and water content to reach saturation.[1][2] A higher dew point indicates more moisture in the air; a dew point greater than 20 °C (68 °F) is considered uncomfortable and greater than 22 °C (72 °F) is considered to be extremely humid." ;
        rdfs:label       "Dew Point Temperature"@en ;
        rdfs:subClassOf  m3-lite:DewPoint .

m3-lite:TrackingClothing
        a                owl:Class ;
        rdfs:comment     ""@en ;
        rdfs:label       "Tracking Clothing"@en ;
        rdfs:subClassOf  m3-lite:TrackingGood .

m3-lite:PresenceStateDriverCard1
        a                owl:Class ;
        rdfs:comment     "Indicates the presence of the first driver card." ;
        rdfs:label       "Presence State Driver Card 1"@en ;
        rdfs:subClassOf  m3-lite:PresenceStateDriverCard .

iot-lite:ActuatingDevice
        a                owl:Class ;
        rdfs:comment     "Actuators (e.g., switch on/off the light)"@en ;
        rdfs:label       "Actuating Device"@en ;
        rdfs:subClassOf  ssn:Device .

m3-lite:Seismometer  a   owl:Class ;
        rdfs:comment     "Seismometers are instruments that measure motions of the ground, including those of seismic waves generated by earthquakes, volcanic eruptions, and other seismic sources."@en ;
        rdfs:label       "Seismometer"@en ;
        rdfs:subClassOf  ssn:SensingDevice .

m3-lite:Magnetometer  a  owl:Class ;
        rdfs:comment     "Magnetic sensors or magnetometer sensors are attached to cupboards to deduce if they are opened or closed"@en ;
        rdfs:label       "Magnetic Sensor"@en ;
        rdfs:subClassOf  ssn:SensingDevice ;
        rdfs:subClassOf  [ a                   owl:Restriction ;
                           owl:onProperty      m3-lite:domainOfInterest ;
                           owl:someValuesFrom  m3-lite:BuildingAutomation
                         ] .

vann:preferredNamespacePrefix
        a       owl:AnnotationProperty .

m3-lite:TrackingAnimal
        a                owl:Class ;
        rdfs:comment     ""@en ;
        rdfs:label       "Tracking Animal"@en ;
        rdfs:subClassOf  m3-lite:TrackingGood .

m3-lite:Microampere  a   owl:Class ;
        rdfs:label       "Microampere (uA)" ;
        rdfs:subClassOf  m3-lite:Ampere .
